scheduler/SchTactics.v
@@ -1,337 +1,551 @@
-(* Require Import CRIS.
+Require Import CRIS wsim_tactics SchHeader SchA.
 
-Require Import SchGInv SchHeader SchA.
-
-Set Implicit Arguments.
-
-Local Open Scope nat_scope.
-
-Section MACROAUX.
-  Import SchAS.
+Section wsim.
   Context `{!invG α Σ Γ, !subG Γ Σ, !sinvG Σ Γ α β τ, !SchAGΣ Σ}.
-  Notation iProp := (iProp Σ).
 
-  (** Sch.spawn *)
+  Local Definition state : Type := alist key Any.t.
+  Local Definition post (R_s R_t : Type) : Type := nat → state * R_s → state * R_t → iProp Σ.
+  Local Definition rel : Type := ∀ R_s R_t : Type,
+    post R_s R_t → bool → bool → nat → state * itree hmodE R_s → state * itree hmodE R_t → iProp Σ.
 
-  Lemma isim_mspawn_hp
-    n contextual fl fr Ist r g {Rs Rt} RR my_tid ps pt nths st_src st_tgt k_src k_tgt scp_src scp_tgt invspc
-    (Stb: string → option fspec) (univ: positive)
-    (fvarg farg: SAny.t) (pre: iProp) (postS: SAny.t → {n & SRFSyn.t n}) 
-    (fn: string) (fsp: fspec) (m: meta fsp)
-    (FINDF: Stb fn = Some fsp)
-    (FINDS: Stb SchName.spawn = Some (SchAS.spawn_spec univ n Stb))
-    (SPWN: ∀ tid, SchAS.fspec_spawnable univ n fsp tid m fvarg↑ farg↑ pre postS)
-    :
-      (((Ist nths st_src st_tgt) ∗ (∃ n, wsats univ n ⊤) ∗ pre) ∗
-      (∀ nths0 st_src0 st_tgt0 tid,
-        ((Ist nths0 st_src0 st_tgt0) ∗ (∃ n, wsats univ n ⊤) ∗ (SchAS.token_th tid postS))
-        -∗ @isim Σ contextual fl fr Ist my_tid r g Rs Rt RR true true nths0 
-              (st_src0, k_src tid)
-              (st_tgt0, k_tgt tid)))
-    ⊢
-      (isim contextual fl fr Ist my_tid r g RR ps pt nths 
-        (st_src, (HMod.sandbox scp_src (interp_smod invspc Stb (Sch.spawn (fn, fvarg)))) >>= k_src)
-        (st_tgt, (HMod.sandbox scp_tgt (PMod.interp (Sch.spawn (fn, farg)))) >>= k_tgt)).
+  Implicit Types r g : rel.
+  Implicit Types ps pt : bool.
+  Implicit Types nths : nat.
+  Implicit Types E : coPset.
+
+  Context (fl_s fl_t : alist string (Any.t → itree hmodE Any.t)).
+  Context (Ist : nat → alist key Any.t → alist key Any.t → iProp Σ).
+  Context (t : option bool).
+  Context (υ ν : univ_id).
+  Context (E : coPset).
+  Context (R_s R_t : Type).
+  Context (RR : post R_s R_t).
+  Context (ps pt : bool).
+  Context (nths : nat).
+  Context (st_s st_t : state).
+
+  Lemma wsim_yield_tgt r g scp_s scp_t ginv spc spc_user k_s k_t
+      (SchInSpc : spc_incl (SchAS.spc υ spc_user) spc) :
+    Ist nths st_s st_t ∗
+    (∀ nths st_s st_t,
+      Ist nths st_s st_t -∗
+      wsim fl_s fl_t Ist (Some true) υ ν ⊤ r g R_s R_t RR false true nths
+        (st_s, (HMod.sandbox scp_s (interp_smod ginv spc Sch.yield)) >>= k_s)
+        (st_t, k_t tt))
+    ⊢ wsim fl_s fl_t Ist (Some true) υ ν ⊤ r g R_s R_t RR ps pt nths
+      (st_s, (HMod.sandbox scp_s (interp_smod ginv spc Sch.yield)) >>= k_s)
+      (st_t, (HMod.sandbox scp_t (PMod.interp Sch.yield)) >>= k_t).
   Proof.
-    iIntros "[(IST & W & PRE) ISIM]". rewrite !/Sch.spawn /ccallU. unseal "Sch".
-    force_l. iSplitR; et. unfold HoareCall. steps_l. force_l.
-    Unshelve.
-    2:{ split.
-      - exact (farg, fvarg, pre, postS).
-      - exists fn. unfold find_fsp. rewrite FINDF. exact m. }
-    force_l ((fn, farg)↑). force_l. iSplitL "PRE W".
-    { iFrame. revert SPWN. revert m. generalize FINDF. unfold find_fsp. rewrite FINDF. i.
-      rewrite (@UIP _ _ _ FINDF0 eq_refl). erewrite <-rew_swap; et. }
-    
-    call "IST"; et.
-    
-    steps_l. steps_r. iDestruct "ASM" as "(W & (% & % & % & % & TKN))". des; subst; hss.
-    steps_r. iApply "ISIM". iFrame.
-  Qed.
+    rewrite !wsim.wsim_eq /wsim.wsim_def.
+    iIntros "SIM P".
+    rewrite /Sch.yield; unseal "Sch".
+    iApply isim_reset. iStopProof.
+    revert nths. combine_quant st_s. combine_quant st_t.
+    eapply isim_coind.
+    iIntros (g' [st_s' [st_t' nths']]) "%MON [[[IST SIM] P] #CIH]". s.
 
-  Lemma isim_mspawn_hh
-    contextual fl fr Ist r g Rs Rt RR my_tid ps pt nths st_src st_tgt k_src k_tgt scp_src scp_tgt invspc_src invspc_tgt
-    (stbf stb_src stb_tgt: string → option fspec) (univ: positive)
-    (fvarg: SAny.t) (fn: string) (fsp: fspec) (m: meta fsp)
-    (FIND: stbf fn = Some fsp)
-    (SPWNS: stb_src SchName.spawn = Some (SchAS.spawn_spec univ stbf))
-    (SPWNT: stb_tgt SchName.spawn = Some (SchAS.spawn_spec univ stbf))
-    :
-      ((Ist nths st_src st_tgt) ∗
-      (∀ nths0 st_src0 st_tgt0 tid,
-        (Ist nths0 st_src0 st_tgt0)
-        -∗ @isim Σ contextual fl fr Ist my_tid r g Rs Rt RR true true nths0 
-              (st_src0, k_src tid)
-              (st_tgt0, k_tgt tid)))
-    ⊢
-      (isim contextual fl fr Ist my_tid r g RR ps pt nths 
-        (st_src, (HMod.sandbox scp_src (interp_smod invspc_src stb_src (Sch.spawn (fn, fvarg))))>>= k_src)
-        (st_tgt, (HMod.sandbox scp_tgt (interp_smod invspc_tgt stb_tgt (Sch.spawn (fn, fvarg)))) >>= k_tgt)).
-  Proof.
-    iIntros "[IST ISIM]". rewrite !/Sch.spawn !/ccallU. unseal "Sch".
-    
-    steps_r. inv SPWNT. ss. iDestruct "GRT" as "[W [% [% GRT]]]". hss.
-    destruct q0. destruct p. destruct p. destruct p. destruct s.
-    iDestruct "GRT" as "((% & % & [% %] & %) & PRE)". des; subst; hss.
-
-    forces_l. iSplit; et. steps_l. forces_l. iSplitL "PRE W".
-    { iFrame. iExists _. iSplit; et. Unshelve.
-      2:{ split; [exact (t, t0, b, o)|]. exists x. ss. }
-      2:exact ((x, t)↑). ss. iSplit; et. }
-
-    call "IST"; et.
-
-    steps_l. iDestruct "ASM" as "[W (% & % & % & [% %] & TKN)]". subst; hss.
-
-    forces_r. iSplitL "TKN W". { iFrame; et. }
-    steps_r. hss. steps_r. iApply "ISIM". iFrame.
-  Qed.
-
-  (** Sch.yield **)
-
-  Lemma isim_myield_tgt_hp
-    contextual fl fr Ist r g {Rs Rt} RR my_tid ps pt nths st_src st_tgt k_src k_tgt scp_src scp_tgt invspc stb univ
-    (SPC: stb SchName.yield = Some (SchAS.yield_spec univ))
-    :
-    bi_entails
-      (((Ist nths st_src st_tgt) ∗ (∃ n, wsats univ n ⊤)) ∗
-      (∀ nths0 st_src0 st_tgt0,
-        ((Ist nths0 st_src0 st_tgt0) ∗ (∃ n, wsats univ n ⊤))
-        -∗ @isim Σ contextual fl fr Ist my_tid r g Rs Rt RR false true nths0 
-              (st_src0, (HMod.sandbox scp_src (interp_smod invspc stb (Sch.yield))) >>= k_src) 
-              (st_tgt0, k_tgt tt)))
-      (isim contextual fl fr Ist my_tid r g RR ps pt nths 
-        (st_src, (HMod.sandbox scp_src (interp_smod invspc stb (Sch.yield))) >>= k_src) 
-        (st_tgt, (HMod.sandbox scp_tgt (PMod.interp (Sch.yield))) >>= k_tgt)).
-  Proof.
-    iIntros "[[IST W] ISIM]". rewrite !/Sch.yield. unseal "Sch".
-    rewrite !unfold_iter_eq. grind. prep. iApply isim_reset.
-    iStopProof. revert st_tgt.
-    combine_quant st_src.
-    combine_quant nths.
-    combine_quant ps.
-    combine_quant pt.
-    eapply isim_coind. ii. destruct a as [pt [ps [nths [st_src st_tgt]]]].
-    iIntros "((IST & W & ISIM) & #CIH)".
-
-    grind. prep. iApply isim_reset. steps_r. destruct q.
-    {
-      steps_r.
-      iApply (isim_mono_knowledge with "[ISIM W IST]").
-      - instantiate (1:=r). et.
-      - instantiate (1:=g). ii. destruct sti_src, sti_tgt. iIntros "G". iModIntro. 
-        iApply H. et.
-      - iApply "ISIM"; iFrame.
+    unfold_iter_r.
+    steps_r. destruct q.
+    { steps_r. iPoseProof ("SIM" with "IST P") as "SIM".
+      iPoseProof (isim_mono_knowledge with "SIM") as "SIM"; cycle 2.
+      { iApply "SIM". }
+      { iIntros (????????) "$"; done. }
+      { iIntros (????????) "P !>"; iApply MON; ss. }
     }
 
-    force_l. instantiate (1:=false). steps_l. unfold ccallU. force_l. iSplitR; et.
-    unfold HoareCall. steps_l. forces_l. iSplitL "W"; et.
-    call "IST"; et. steps_l. iDestruct "ASM" as "(W & % & %)". subst; hss. steps_r. hss. steps_r. steps_l.
-
-    rewrite !unfold_iter_eq. grind. prep. prep. by_coind "CIH"; iFrame; et.
-
-    Unshelve. all: ss.
+    steps_r.
+    unfold_iter_l; steps_l.
+    force_l false; steps_l.
+    forces_l. iSplitL "P"; first (ss; eauto).
+    steps_l. call "IST"; ss.
+    steps_l. iDestruct "ASM" as "[P [-> ->]]". hss. steps_l.
+    steps_r. hss. steps_r.
+    iApply isim_progress; iApply isim_base.
+    iSpecialize ("CIH" $! _);
+    (hrepeat do 1 first[instantiate (1:= (_,_))|instantiate (1:= existT _ _)]); s;
+    iApply "CIH".
+    iFrame.
+    Unshelve. done.
   Qed.
 
-  Lemma isim_myield_tgt_hh
-    contextual fl fr Ist r g {Rs Rt} RR my_tid ps pt nths st_src st_tgt k_src k_tgt scp_src scp_tgt invspc stb univ
-    (SPC: stb SchName.yield = Some (SchAS.yield_spec univ))
-    :
-    bi_entails
-      ((Ist nths st_src st_tgt) ∗
-      (∀ nths0 st_src0 st_tgt0,
-        (Ist nths0 st_src0 st_tgt0)
-        -∗ @isim Σ contextual fl fr Ist my_tid r g Rs Rt RR false true nths0 
-              (st_src0, (HMod.sandbox scp_src (interp_smod invspc stb (Sch.yield))) >>= k_src) 
-              (st_tgt0, k_tgt tt)))
-      (isim contextual fl fr Ist my_tid r g RR ps pt nths 
-        (st_src, (HMod.sandbox scp_src (interp_smod invspc stb (Sch.yield))) >>= k_src) 
-        (st_tgt, (HMod.sandbox scp_tgt (interp_smod invspc stb (Sch.yield))) >>= k_tgt)).
+  Lemma wsim_yield_src r g scp_s ginv spc spc_user k_s i_t
+      (SchInSpc : spc_incl (SchAS.spc υ spc_user) spc) :
+    wsim fl_s fl_t Ist (Some true) υ ν E r g R_s R_t RR true pt nths
+      (st_s, k_s tt)
+      (st_t, i_t)
+    ⊢ wsim fl_s fl_t Ist (Some true) υ ν E r g R_s R_t RR ps pt nths
+      (st_s, (HMod.sandbox scp_s (interp_smod ginv spc Sch.yield)) >>= k_s)
+      (st_t, i_t).
   Proof.
-    iIntros "[IST ISIM]". rewrite !/Sch.yield. unseal "Sch".
-    rewrite !unfold_iter_eq. grind. prep. iApply isim_reset.
-    iStopProof. revert st_tgt.
-    combine_quant st_src.
-    combine_quant nths.
-    combine_quant ps.
-    combine_quant pt.
-    eapply isim_coind. ii. destruct a as [pt [ps [nths [st_src st_tgt]]]].
-    iIntros "((IST & ISIM) & #CIH)".
+    iIntros "SIM".
+    rewrite /Sch.yield; unseal "Sch".
+    unfold_iter_l; wsteps_l.
+    wforce_l true; wsteps_l. iApply "SIM".
+  Qed.
 
-    grind. prep. iApply isim_reset. steps_r. destruct q.
-    {
-      steps_r.
-      iApply (isim_mono_knowledge with "[ISIM IST]").
-      - instantiate (1:=r). et.
-      - instantiate (1:=g). ii. destruct sti_src, sti_tgt. iIntros "G". iModIntro. 
-        iApply H. et.
-      - iApply "ISIM"; iFrame.
+  Lemma wsim_spawn fn args fn_spec (x : meta fn_spec) (P : iProp Σ) (Q : SAny.t → SynDepO)
+      r g scp_s scp_t ginv spc spc_user k_s k_t
+      (SchInSpc : spc_incl (SchAS.spc υ spc_user) spc)
+      (CalleeInSpc : spc_user fn = Some fn_spec)
+      (Spawnable : SchAS.fspec_spawnable υ fn_spec x args↑ args↑ P Q) :
+    Ist nths st_s st_t ∗
+    P ∗
+    (∀ tid nths st_s st_t,
+        Ist nths st_s st_t
+        -∗ SchAS.token_th tid Q
+        -∗ wsim fl_s fl_t Ist (Some true) υ ν ⊤ r g R_s R_t RR true true nths
+            (st_s, k_s tid) (st_t, k_t tid))
+    ⊢ wsim fl_s fl_t Ist (Some true) υ ν ⊤ r g R_s R_t RR ps pt nths
+      (st_s, (HMod.sandbox scp_s (interp_smod ginv spc (Sch.spawn (fn, args)))) >>= k_s)
+      (st_t, (HMod.sandbox scp_t (PMod.interp (Sch.spawn (fn, args)))) >>= k_t).
+  Proof.
+    iIntros "(I & P & SIM)". rewrite /Sch.spawn; unseal "Sch".
+    wsteps_l. wforces_l. iSplitL "P".
+    { iExists _; iSplit; eauto.
+      Unshelve.
+      2:{ split; first exact (args, args, P, Q).
+          exists fn. rewrite /find_fsp CalleeInSpc; exact x.
+      }
+      2:{ exact ((fn, args)↑). }
+      { ss; iFrame; iPureIntro. do 3 split; eauto.
+        rewrite /find_fsp. generalize (CalleeInSpc). rewrite CalleeInSpc.
+        intros H; rewrite (UIP_refl _ _ H) /eq_rect_r /=. done.
+      }
     }
-
-    steps_r. inv SPC. ss. unfold precond. ss. iDestruct "GRT" as "[W %]". des; subst; hss.
-
-    force_l. instantiate (1:=false). steps_l. unfold ccallU. force_l. iSplitR; et.
-    unfold HoareCall. steps_l. forces_l. iSplitL "W"; et.
-    call "IST"; et.
-    
-    steps_l. iDestruct "ASM" as "(W & % & %)". subst; hss. steps_r. hss. steps_r. steps_l.
-
-    forces_r. iSplitL "W"; et. steps_r. hss. steps_r.
-
-    rewrite !unfold_iter_eq. grind. prep. prep. by_coind "CIH"; iFrame; et.
-
-    Unshelve. all: ss.
+    wsteps_l. wsteps_r. wcall "I". wsteps_l. wsteps_r.
+    iDestruct "ASM" as "[%vr [-> [%tid [[-> ->] TKN]]]]". hss. wsteps_r.
+    iApply ("SIM" with "IST TKN").
   Qed.
 
-  Lemma isim_myield_src
-    contextual fl fr Ist r g {Rs Rt} RR my_tid ps pt nths st_src st_tgt k_src i_tgt scp_src invspc stb univ
-    (SPC: stb SchName.yield = Some (SchAS.yield_spec univ))
-    :
-    bi_entails
-      (((Ist nths st_src st_tgt) ∗ (∃ n, wsats univ n ⊤)) ∗
-      (∀ nths0 st_src0 st_tgt0,
-        ((Ist nths0 st_src0 st_tgt0) ∗ (∃ n, wsats univ n ⊤))
-        -∗ @isim Σ contextual fl fr Ist my_tid r g Rs Rt RR true false nths0 
-              (st_src0, k_src tt) 
-              (st_tgt0, i_tgt)))
-      (isim contextual fl fr Ist my_tid r g RR ps pt nths 
-        (st_src, (HMod.sandbox scp_src (interp_smod invspc stb (Sch.yield))) >>= k_src) 
-        (st_tgt, i_tgt)).
+  Lemma wsim_join tid (Q : SAny.t → SynDepO) R
+      r g scp_s scp_t ginv spc spc_user k_s k_t
+      (SchInSpc : spc_incl (SchAS.spc υ spc_user) spc) :
+    Ist nths st_s st_t ∗
+    SchAS.token_th tid Q ∗
+    (∀ nths st_s st_t ret,
+        Ist nths st_s st_t
+        -∗ interp_cond (Q ret↑↑)
+        -∗ wsim fl_s fl_t Ist (Some true) υ ν ⊤ r g R_s R_t RR true true nths
+            (st_s, k_s ret) (st_t, k_t ret))
+    ⊢ wsim fl_s fl_t Ist (Some true) υ ν ⊤ r g R_s R_t RR ps pt nths
+      (st_s, (HMod.sandbox scp_s (interp_smod ginv spc (Sch.join R tid))) >>= k_s)
+      (st_t, (HMod.sandbox scp_t (PMod.interp (Sch.join R tid))) >>= k_t).
   Proof.
-    iIntros "[[IST W] ISIM]". rewrite !/Sch.yield. unseal "Sch".
-    rewrite !unfold_iter_eq. grind. prep. iApply isim_reset.
-    force_l. instantiate (1:=true). steps_l. iApply "ISIM"; iFrame.
+    iIntros "(IST & TK & SIM)". rewrite /Sch.join; unseal "Sch".
+    wsteps_l. wforce_l (tid, Q). wsteps_l. wforce_l (tid↑). wsteps_l. wforce_l.
+    iFrame; iSplit; eauto. wsteps_l.
+
+    wsteps_r. wcall "IST". wsteps_l. iDestruct "ASM" as "[[%ret' [-> Q]] ->]". hss.
+    wsteps_r. hss. wsteps_r.
+    apply SAny.downcast_upcast in G0. inv G0. rewrite SAny.upcast_downcast. hss. wstep_r.
+    iApply ("SIM" with "IST Q").
   Qed.
+End wsim.
 
-  (* Sch.join *)
-  
-  Lemma isim_mjoin_hp
-    contextual fl fr Ist r g {Rs Rt} RR my_tid ps pt nths st_src st_tgt RT (k_src: RT → itree hmodE Rs) (k_tgt: RT → itree hmodE Rt)
-    scp_src scp_tgt invspc tid
-    (Stb: string → option fspec) (univ: positive) (postS: SAny.t → {n & SRFSyn.t n})
-    (FINDS: Stb SchName.join = Some (SchAS.join_spec univ))
-    :
-      (((Ist nths st_src st_tgt) ∗ (∃ n, wsats univ n ⊤) ∗ (SchAS.token_th tid postS)) ∗
-      (∀ nths0 st_src0 st_tgt0 (ret: RT),
-        ((Ist nths0 st_src0 st_tgt0) ∗ (∃ n, wsats univ n ⊤) ∗ (interp_cond (postS ret↑↑)))
-        -∗ @isim Σ contextual fl fr Ist my_tid r g Rs Rt RR true true nths0 
-              (st_src0, k_src ret)
-              (st_tgt0, k_tgt ret)))
-    ⊢
-      (isim contextual fl fr Ist my_tid r g RR ps pt nths 
-        (st_src, (HMod.sandbox scp_src (interp_smod invspc Stb (Sch.join RT tid))) >>= k_src)
-        (st_tgt, (HMod.sandbox scp_tgt (PMod.interp (Sch.join RT tid))) >>= k_tgt)).
-  Proof.
-    iIntros "[(IST & W & TKN) ISIM]". rewrite !/Sch.join !/ccallU. unseal "Sch".
-    force_l. iSplitR; et. unfold HoareCall. steps_l. force_l (tid, postS).
-    force_l (tid↑). force_l. iSplitL "TKN W"; iFrame; et.
-    call "IST"; et.
-    
-    steps_l. steps_r. iDestruct "ASM" as "(W & [% [% POST]] & %)". des; subst; hss.
-    steps_r. apply SAny.downcast_upcast in G0. r in G0. subst.
-    rewrite SAny.upcast_downcast. hss. steps_r.
-    
-    iApply "ISIM". iFrame.
-  Qed.
-
-  Lemma isim_mjoin_hh
-    contextual fl fr Ist r g {Rs Rt} RR my_tid ps pt nths st_src st_tgt RT (k_src: RT → itree hmodE Rs) (k_tgt: RT → itree hmodE Rt)
-    scp_src scp_tgt invspc_src invspc_tgt univ stb_src stb_tgt tid
-    (JOINS: stb_src SchName.join = Some (SchAS.join_spec univ))
-    (JOINT: stb_tgt SchName.join = Some (SchAS.join_spec univ))
-    :
-      ((Ist nths st_src st_tgt) ∗
-      (∀ nths0 st_src0 st_tgt0 (ret: RT),
-        (Ist nths0 st_src0 st_tgt0)
-        -∗ @isim Σ contextual fl fr Ist my_tid r g Rs Rt RR true true nths0 
-              (st_src0, k_src ret)
-              (st_tgt0, k_tgt ret)))
-    ⊢
-      (isim contextual fl fr Ist my_tid r g RR ps pt nths 
-        (st_src, (HMod.sandbox scp_src (interp_smod invspc_src stb_src (Sch.join RT tid)))>>= k_src)
-        (st_tgt, (HMod.sandbox scp_tgt (interp_smod invspc_tgt stb_tgt (Sch.join RT tid))) >>= k_tgt)).
-  Proof.
-    iIntros "[IST ISIM]". rewrite !/Sch.join !/ccallU. unseal "Sch".
-    
-    steps_r. inv JOINT. ss. iDestruct "GRT" as "[W PRE]". unfold precond. hss.
-    destruct q0. ss. iDestruct "PRE" as "[[% TKN] %]". des; subst; hss.
-
-    forces_l. iSplit; et. steps_l. force_l (n, o). forces_l. iSplitL "TKN W"; iFrame; et.
-    
-    call "IST"; et.
-
-    steps_l. iDestruct "ASM" as "[W [[% [% POST]] %]]". subst; hss.
-    apply SAny.downcast_upcast in G1. r in G1. subst.
-
-    forces_r. iSplitL "POST W". { iFrame; et. }
-    steps_r. hss. steps_r. rewrite SAny.upcast_downcast. hss. steps_r.
-    iApply "ISIM". iFrame.
-  Qed.
-
-End MACROAUX.
-
-Local Ltac _prep_macro_l :=
-  prep; match goal with
-  | [|- context[interp_smod _ _ (Sch.spawn _ >>= _)]] =>
-      rewrite// [in (interp_smod _ _ (Sch.spawn _ >>= _))] SModRed.interp_bind; _prep_macro_l
+Local Ltac _prep_macro :=
+  ired;
+  match goal with
+  | [|- context[HMod.sandbox _ (interp_smod _ _ (Sch.spawn _)) >>= _]] => fail 1
   | [|- context[HMod.sandbox _ (interp_smod _ _ (Sch.spawn _) >>= _)]] =>
       rewrite// [in HMod.sandbox _ (interp_smod _ _ (Sch.spawn _) >>= _)] HModSB.transl_bind
-  | [|- context[interp_smod _ _ (Sch.yield >>= _)]] =>
-      rewrite// [in (interp_smod _ _ (Sch.yield >>= _))] SModRed.interp_bind; _prep_macro_l
+  | [|- context[interp_smod _ _ (Sch.spawn _ >>= _)]] =>
+      rewrite// [in (interp_smod _ _ (Sch.spawn _ >>= _))] SModRed.interp_bind; _prep_macro
+  | [|- context[HMod.sandbox _ (interp_smod _ _ (Sch.yield)) >>= _]] => fail 1
   | [|- context[HMod.sandbox _ (interp_smod _ _ (Sch.yield) >>= _)]] =>
       rewrite// [in HMod.sandbox _ (interp_smod _ _ (Sch.yield) >>= _)] HModSB.transl_bind
-  | [|- context[interp_smod _ _ (Sch.join _ _ >>= _)]] =>
-      rewrite// [in (interp_smod _ _ (Sch.join _ _ >>= _))] SModRed.interp_bind; _prep_macro_l
+  | [|- context[interp_smod _ _ (Sch.yield >>= _)]] =>
+      rewrite// [in (interp_smod _ _ (Sch.yield >>= _))] SModRed.interp_bind; _prep_macro
+  | [|- context[HMod.sandbox _ (interp_smod _ _ (Sch.join _ _)) >>= _]] => fail 1
   | [|- context[HMod.sandbox _ (interp_smod _ _ (Sch.join _ _) >>= _)]] =>
       rewrite// [in HMod.sandbox _ (interp_smod _ _ (Sch.join _ _) >>= _)] HModSB.transl_bind
-  end; prep.
-
-Local Ltac _prep_macro_r :=
-  prep; match goal with
-  | [|- context[PMod.interp (Sch.spawn _ >>= _)]] =>
-      rewrite// [in (PMod.interp (Sch.spawn _ >>= _))] PModRed.interp_bind; _prep_macro_r
+  | [|- context[interp_smod _ _ (Sch.join _ _ >>= _)]] =>
+      rewrite// [in (interp_smod _ _ (Sch.join _ _ >>= _))] SModRed.interp_bind; _prep_macro
+  | [|- context[HMod.sandbox _ (PMod.interp (Sch.spawn _)) >>= _]] => fail 1
   | [|- context[HMod.sandbox _ (PMod.interp (Sch.spawn _) >>= _)]] =>
       rewrite// [in HMod.sandbox _ (PMod.interp (Sch.spawn _) >>= _)] HModSB.transl_bind
-  | [|- context[PMod.interp (Sch.yield >>= _)]] =>
-      rewrite// [in (PMod.interp (Sch.yield >>= _))] PModRed.interp_bind; _prep_macro_r
+  | [|- context[PMod.interp (Sch.spawn _ >>= _)]] =>
+      rewrite// [in (PMod.interp (Sch.spawn _ >>= _))] PModRed.interp_bind; _prep_macro
+  | [|- context[HMod.sandbox _ (PMod.interp (Sch.yield)) >>= _]] => fail 1
   | [|- context[HMod.sandbox _ (PMod.interp (Sch.yield) >>= _)]] =>
       rewrite// [in HMod.sandbox _ (PMod.interp (Sch.yield) >>= _)] HModSB.transl_bind
-  | [|- context[PMod.interp (Sch.join _ _ >>= _)]] =>
-      rewrite// [in (PMod.interp (Sch.join _ _ >>= _))] PModRed.interp_bind; _prep_macro_r
+  | [|- context[PMod.interp (Sch.yield >>= _)]] =>
+      rewrite// [in (PMod.interp (Sch.yield >>= _))] PModRed.interp_bind; _prep_macro
+  | [|- context[HMod.sandbox _ (PMod.interp (Sch.join _ _)) >>= _]] => fail 1
   | [|- context[HMod.sandbox _ (PMod.interp (Sch.join _ _) >>= _)]] =>
       rewrite// [in HMod.sandbox _ (PMod.interp (Sch.join _ _) >>= _)] HModSB.transl_bind
-  end; prep.
+  | [|- context[PMod.interp (Sch.join _ _ >>= _)]] =>
+      rewrite// [in (PMod.interp (Sch.join _ _ >>= _))] PModRed.interp_bind; _prep_macro
+  end.
+
+Local Ltac prep_macro_l :=
+  let marker := fresh "MARKER" in
+  set_marker marker;
+  hide_ihyps;
+  hide_itree_r;
+  try _prep_macro; ired;
+  show_until marker.  
+
+Local Ltac prep_macro_r :=
+  let marker := fresh "MARKER" in
+  set_marker marker;
+  hide_ihyps;
+  hide_itree_l;
+  try _prep_macro; ired;
+  show_until marker.
 
 Local Ltac prep_macro :=
   let marker := fresh "MARKER" in
-  hide_itree_r marker; try _prep_macro_l; show_itree marker;
-  hide_itree_l marker; try _prep_macro_r; show_itree marker.
+  set_marker marker;
+  hide_ihyps;
+  hide_itree_r; try _prep_macro; ired; show_itree;
+  hide_itree_l; try _prep_macro; ired; show_itree;
+  show_until marker.
 
-Ltac yield_r hyps :=
-  prep_macro;
-  first [
-    iApply isim_myield_tgt_hp; des_pairs; s;
-    [|iSplitL hyps; [|iIntros "% % %"; iIntros "[IST W]"]] |
-    iApply isim_myield_tgt_hh; des_pairs; s;
-    [|iSplitL hyps; [|iIntros "% % %"; iIntros "IST"]]].
+Ltac sch_yield_l :=
+  prep_macro; iApply wsim_yield_src; first eassumption.
 
-Ltac yield_l hyps :=
-  prep_macro;
-  iApply isim_myield_src; des_pairs; s;
-  [|iSplitL hyps; [ |iIntros "% % %"; iIntros "[IST W]"]].
+Ltac sch_yield_r :=
+  prep_macro; iApply wsim_yield_tgt; first eassumption.
 
-Ltac spawn hyps :=
-  prep_macro;
-  first [
-    iApply isim_mspawn_hp; des_pairs; s;
-    [| | |iSplitL hyps; [|iIntros "% % % %"; iIntros "[IST [W TKN]]"]] |
-    iApply isim_mspawn_hh; des_pairs; s;
-    [| | |iSplitL hyps; [|iIntros "% % % %"; iIntros "IST"]]].
+Ltac sch_spawn :=
+  prep_macro; iApply wsim_spawn; first eassumption.
 
-Ltac join hyps :=
-  prep_macro;
-  first [
-    iApply isim_mjoin_hp; des_pairs; s;
-    [|iSplitL hyps; [|iIntros "% % % %"; iIntros "[IST [W POST]]"]] |
-    iApply isim_mjoin_hh; des_pairs; s;
-    [| |iSplitL hyps; [|iIntros "% % % %"; iIntros "IST"]]]. *)
+Ltac sch_join :=
+  prep_macro; iApply wsim_join; first eassumption.
+
+
+
+
+
+
+
+
+(* Section MACROAUX. *)
+(*   Import SchAS. *)
+(*   Context `{!invG α Σ Γ, !subG Γ Σ, !sinvG Σ Γ α β τ, !SchAGΣ Σ}. *)
+(*   Notation iProp := (iProp Σ). *)
+
+(*   (** Sch.spawn *) *)
+
+(*   Lemma isim_mspawn_hp *)
+(*     n contextual fl fr Ist r g {Rs Rt} RR my_tid ps pt nths st_src st_tgt k_src k_tgt scp_src scp_tgt invspc *)
+(*     (Stb: string → option fspec) (univ: positive) *)
+(*     (fvarg farg: SAny.t) (pre: iProp) (postS: SAny.t → {n & SRFSyn.t n})  *)
+(*     (fn: string) (fsp: fspec) (m: meta fsp) *)
+(*     (FINDF: Stb fn = Some fsp) *)
+(*     (FINDS: Stb SchName.spawn = Some (SchAS.spawn_spec univ n Stb)) *)
+(*     (SPWN: ∀ tid, SchAS.fspec_spawnable univ n fsp tid m fvarg↑ farg↑ pre postS) *)
+(*     : *)
+(*       (((Ist nths st_src st_tgt) ∗ (∃ n, wsats univ n ⊤) ∗ pre) ∗ *)
+(*       (∀ nths0 st_src0 st_tgt0 tid, *)
+(*         ((Ist nths0 st_src0 st_tgt0) ∗ (∃ n, wsats univ n ⊤) ∗ (SchAS.token_th tid postS)) *)
+(*         -∗ @isim Σ contextual fl fr Ist my_tid r g Rs Rt RR true true nths0  *)
+(*               (st_src0, k_src tid) *)
+(*               (st_tgt0, k_tgt tid))) *)
+(*     ⊢ *)
+(*       (isim contextual fl fr Ist my_tid r g RR ps pt nths  *)
+(*         (st_src, (HMod.sandbox scp_src (interp_smod invspc Stb (Sch.spawn (fn, fvarg)))) >>= k_src) *)
+(*         (st_tgt, (HMod.sandbox scp_tgt (PMod.interp (Sch.spawn (fn, farg)))) >>= k_tgt)). *)
+(*   Proof. *)
+(*     iIntros "[(IST & W & PRE) ISIM]". rewrite !/Sch.spawn /ccallU. unseal "Sch". *)
+(*     force_l. iSplitR; et. unfold HoareCall. steps_l. force_l. *)
+(*     Unshelve. *)
+(*     2:{ split. *)
+(*       - exact (farg, fvarg, pre, postS). *)
+(*       - exists fn. unfold find_fsp. rewrite FINDF. exact m. } *)
+(*     force_l ((fn, farg)↑). force_l. iSplitL "PRE W". *)
+(*     { iFrame. revert SPWN. revert m. generalize FINDF. unfold find_fsp. rewrite FINDF. i. *)
+(*       rewrite (@UIP _ _ _ FINDF0 eq_refl). erewrite <-rew_swap; et. } *)
+    
+(*     call "IST"; et. *)
+    
+(*     steps_l. steps_r. iDestruct "ASM" as "(W & (% & % & % & % & TKN))". des; subst; hss. *)
+(*     steps_r. iApply "ISIM". iFrame. *)
+(*   Qed. *)
+
+(*   Lemma isim_mspawn_hh *)
+(*     contextual fl fr Ist r g Rs Rt RR my_tid ps pt nths st_src st_tgt k_src k_tgt scp_src scp_tgt invspc_src invspc_tgt *)
+(*     (stbf stb_src stb_tgt: string → option fspec) (univ: positive) *)
+(*     (fvarg: SAny.t) (fn: string) (fsp: fspec) (m: meta fsp) *)
+(*     (FIND: stbf fn = Some fsp) *)
+(*     (SPWNS: stb_src SchName.spawn = Some (SchAS.spawn_spec univ stbf)) *)
+(*     (SPWNT: stb_tgt SchName.spawn = Some (SchAS.spawn_spec univ stbf)) *)
+(*     : *)
+(*       ((Ist nths st_src st_tgt) ∗ *)
+(*       (∀ nths0 st_src0 st_tgt0 tid, *)
+(*         (Ist nths0 st_src0 st_tgt0) *)
+(*         -∗ @isim Σ contextual fl fr Ist my_tid r g Rs Rt RR true true nths0  *)
+(*               (st_src0, k_src tid) *)
+(*               (st_tgt0, k_tgt tid))) *)
+(*     ⊢ *)
+(*       (isim contextual fl fr Ist my_tid r g RR ps pt nths  *)
+(*         (st_src, (HMod.sandbox scp_src (interp_smod invspc_src stb_src (Sch.spawn (fn, fvarg))))>>= k_src) *)
+(*         (st_tgt, (HMod.sandbox scp_tgt (interp_smod invspc_tgt stb_tgt (Sch.spawn (fn, fvarg)))) >>= k_tgt)). *)
+(*   Proof. *)
+(*     iIntros "[IST ISIM]". rewrite !/Sch.spawn !/ccallU. unseal "Sch". *)
+    
+(*     steps_r. inv SPWNT. ss. iDestruct "GRT" as "[W [% [% GRT]]]". hss. *)
+(*     destruct q0. destruct p. destruct p. destruct p. destruct s. *)
+(*     iDestruct "GRT" as "((% & % & [% %] & %) & PRE)". des; subst; hss. *)
+
+(*     forces_l. iSplit; et. steps_l. forces_l. iSplitL "PRE W". *)
+(*     { iFrame. iExists _. iSplit; et. Unshelve. *)
+(*       2:{ split; [exact (t, t0, b, o)|]. exists x. ss. } *)
+(*       2:exact ((x, t)↑). ss. iSplit; et. } *)
+
+(*     call "IST"; et. *)
+
+(*     steps_l. iDestruct "ASM" as "[W (% & % & % & [% %] & TKN)]". subst; hss. *)
+
+(*     forces_r. iSplitL "TKN W". { iFrame; et. } *)
+(*     steps_r. hss. steps_r. iApply "ISIM". iFrame. *)
+(*   Qed. *)
+
+(*   (** Sch.yield **) *)
+
+(*   Lemma isim_myield_tgt_hp *)
+(*     contextual fl fr Ist r g {Rs Rt} RR my_tid ps pt nths st_src st_tgt k_src k_tgt scp_src scp_tgt invspc stb univ *)
+(*     (SPC: stb SchName.yield = Some (SchAS.yield_spec univ)) *)
+(*     : *)
+(*     bi_entails *)
+(*       (((Ist nths st_src st_tgt) ∗ (∃ n, wsats univ n ⊤)) ∗ *)
+(*       (∀ nths0 st_src0 st_tgt0, *)
+(*         ((Ist nths0 st_src0 st_tgt0) ∗ (∃ n, wsats univ n ⊤)) *)
+(*         -∗ @isim Σ contextual fl fr Ist my_tid r g Rs Rt RR false true nths0  *)
+(*               (st_src0, (HMod.sandbox scp_src (interp_smod invspc stb (Sch.yield))) >>= k_src)  *)
+(*               (st_tgt0, k_tgt tt))) *)
+(*       (isim contextual fl fr Ist my_tid r g RR ps pt nths  *)
+(*         (st_src, (HMod.sandbox scp_src (interp_smod invspc stb (Sch.yield))) >>= k_src)  *)
+(*         (st_tgt, (HMod.sandbox scp_tgt (PMod.interp (Sch.yield))) >>= k_tgt)). *)
+(*   Proof. *)
+(*     iIntros "[[IST W] ISIM]". rewrite !/Sch.yield. unseal "Sch". *)
+(*     rewrite !unfold_iter_eq. grind. prep. iApply isim_reset. *)
+(*     iStopProof. revert st_tgt. *)
+(*     combine_quant st_src. *)
+(*     combine_quant nths. *)
+(*     combine_quant ps. *)
+(*     combine_quant pt. *)
+(*     eapply isim_coind. ii. destruct a as [pt [ps [nths [st_src st_tgt]]]]. *)
+(*     iIntros "((IST & W & ISIM) & #CIH)". *)
+
+(*     grind. prep. iApply isim_reset. steps_r. destruct q. *)
+(*     { *)
+(*       steps_r. *)
+(*       iApply (isim_mono_knowledge with "[ISIM W IST]"). *)
+(*       - instantiate (1:=r). et. *)
+(*       - instantiate (1:=g). ii. destruct sti_src, sti_tgt. iIntros "G". iModIntro.  *)
+(*         iApply H. et. *)
+(*       - iApply "ISIM"; iFrame. *)
+(*     } *)
+
+(*     force_l. instantiate (1:=false). steps_l. unfold ccallU. force_l. iSplitR; et. *)
+(*     unfold HoareCall. steps_l. forces_l. iSplitL "W"; et. *)
+(*     call "IST"; et. steps_l. iDestruct "ASM" as "(W & % & %)". subst; hss. steps_r. hss. steps_r. steps_l. *)
+
+(*     rewrite !unfold_iter_eq. grind. prep. prep. by_coind "CIH"; iFrame; et. *)
+
+(*     Unshelve. all: ss. *)
+(*   Qed. *)
+
+(*   Lemma isim_myield_tgt_hh *)
+(*     contextual fl fr Ist r g {Rs Rt} RR my_tid ps pt nths st_src st_tgt k_src k_tgt scp_src scp_tgt invspc stb univ *)
+(*     (SPC: stb SchName.yield = Some (SchAS.yield_spec univ)) *)
+(*     : *)
+(*     bi_entails *)
+(*       ((Ist nths st_src st_tgt) ∗ *)
+(*       (∀ nths0 st_src0 st_tgt0, *)
+(*         (Ist nths0 st_src0 st_tgt0) *)
+(*         -∗ @isim Σ contextual fl fr Ist my_tid r g Rs Rt RR false true nths0  *)
+(*               (st_src0, (HMod.sandbox scp_src (interp_smod invspc stb (Sch.yield))) >>= k_src)  *)
+(*               (st_tgt0, k_tgt tt))) *)
+(*       (isim contextual fl fr Ist my_tid r g RR ps pt nths  *)
+(*         (st_src, (HMod.sandbox scp_src (interp_smod invspc stb (Sch.yield))) >>= k_src)  *)
+(*         (st_tgt, (HMod.sandbox scp_tgt (interp_smod invspc stb (Sch.yield))) >>= k_tgt)). *)
+(*   Proof. *)
+(*     iIntros "[IST ISIM]". rewrite !/Sch.yield. unseal "Sch". *)
+(*     rewrite !unfold_iter_eq. grind. prep. iApply isim_reset. *)
+(*     iStopProof. revert st_tgt. *)
+(*     combine_quant st_src. *)
+(*     combine_quant nths. *)
+(*     combine_quant ps. *)
+(*     combine_quant pt. *)
+(*     eapply isim_coind. ii. destruct a as [pt [ps [nths [st_src st_tgt]]]]. *)
+(*     iIntros "((IST & ISIM) & #CIH)". *)
+
+(*     grind. prep. iApply isim_reset. steps_r. destruct q. *)
+(*     { *)
+(*       steps_r. *)
+(*       iApply (isim_mono_knowledge with "[ISIM IST]"). *)
+(*       - instantiate (1:=r). et. *)
+(*       - instantiate (1:=g). ii. destruct sti_src, sti_tgt. iIntros "G". iModIntro.  *)
+(*         iApply H. et. *)
+(*       - iApply "ISIM"; iFrame. *)
+(*     } *)
+
+(*     steps_r. inv SPC. ss. unfold precond. ss. iDestruct "GRT" as "[W %]". des; subst; hss. *)
+
+(*     force_l. instantiate (1:=false). steps_l. unfold ccallU. force_l. iSplitR; et. *)
+(*     unfold HoareCall. steps_l. forces_l. iSplitL "W"; et. *)
+(*     call "IST"; et. *)
+    
+(*     steps_l. iDestruct "ASM" as "(W & % & %)". subst; hss. steps_r. hss. steps_r. steps_l. *)
+
+(*     forces_r. iSplitL "W"; et. steps_r. hss. steps_r. *)
+
+(*     rewrite !unfold_iter_eq. grind. prep. prep. by_coind "CIH"; iFrame; et. *)
+
+(*     Unshelve. all: ss. *)
+(*   Qed. *)
+
+(*   Lemma isim_myield_src *)
+(*     contextual fl fr Ist r g {Rs Rt} RR my_tid ps pt nths st_src st_tgt k_src i_tgt scp_src invspc stb univ *)
+(*     (SPC: stb SchName.yield = Some (SchAS.yield_spec univ)) *)
+(*     : *)
+(*     bi_entails *)
+(*       (((Ist nths st_src st_tgt) ∗ (∃ n, wsats univ n ⊤)) ∗ *)
+(*       (∀ nths0 st_src0 st_tgt0, *)
+(*         ((Ist nths0 st_src0 st_tgt0) ∗ (∃ n, wsats univ n ⊤)) *)
+(*         -∗ @isim Σ contextual fl fr Ist my_tid r g Rs Rt RR true false nths0  *)
+(*               (st_src0, k_src tt)  *)
+(*               (st_tgt0, i_tgt))) *)
+(*       (isim contextual fl fr Ist my_tid r g RR ps pt nths  *)
+(*         (st_src, (HMod.sandbox scp_src (interp_smod invspc stb (Sch.yield))) >>= k_src)  *)
+(*         (st_tgt, i_tgt)). *)
+(*   Proof. *)
+(*     iIntros "[[IST W] ISIM]". rewrite !/Sch.yield. unseal "Sch". *)
+(*     rewrite !unfold_iter_eq. grind. prep. iApply isim_reset. *)
+(*     force_l. instantiate (1:=true). steps_l. iApply "ISIM"; iFrame. *)
+(*   Qed. *)
+
+(*   (* Sch.join *) *)
+  
+(*   Lemma isim_mjoin_hp *)
+(*     contextual fl fr Ist r g {Rs Rt} RR my_tid ps pt nths st_src st_tgt RT (k_src: RT → itree hmodE Rs) (k_tgt: RT → itree hmodE Rt) *)
+(*     scp_src scp_tgt invspc tid *)
+(*     (Stb: string → option fspec) (univ: positive) (postS: SAny.t → {n & SRFSyn.t n}) *)
+(*     (FINDS: Stb SchName.join = Some (SchAS.join_spec univ)) *)
+(*     : *)
+(*       (((Ist nths st_src st_tgt) ∗ (∃ n, wsats univ n ⊤) ∗ (SchAS.token_th tid postS)) ∗ *)
+(*       (∀ nths0 st_src0 st_tgt0 (ret: RT), *)
+(*         ((Ist nths0 st_src0 st_tgt0) ∗ (∃ n, wsats univ n ⊤) ∗ (interp_cond (postS ret↑↑))) *)
+(*         -∗ @isim Σ contextual fl fr Ist my_tid r g Rs Rt RR true true nths0  *)
+(*               (st_src0, k_src ret) *)
+(*               (st_tgt0, k_tgt ret))) *)
+(*     ⊢ *)
+(*       (isim contextual fl fr Ist my_tid r g RR ps pt nths  *)
+(*         (st_src, (HMod.sandbox scp_src (interp_smod invspc Stb (Sch.join RT tid))) >>= k_src) *)
+(*         (st_tgt, (HMod.sandbox scp_tgt (PMod.interp (Sch.join RT tid))) >>= k_tgt)). *)
+(*   Proof. *)
+(*     iIntros "[(IST & W & TKN) ISIM]". rewrite !/Sch.join !/ccallU. unseal "Sch". *)
+(*     force_l. iSplitR; et. unfold HoareCall. steps_l. force_l (tid, postS). *)
+(*     force_l (tid↑). force_l. iSplitL "TKN W"; iFrame; et. *)
+(*     call "IST"; et. *)
+    
+(*     steps_l. steps_r. iDestruct "ASM" as "(W & [% [% POST]] & %)". des; subst; hss. *)
+(*     steps_r. apply SAny.downcast_upcast in G0. r in G0. subst. *)
+(*     rewrite SAny.upcast_downcast. hss. steps_r. *)
+    
+(*     iApply "ISIM". iFrame. *)
+(*   Qed. *)
+
+(*   Lemma isim_mjoin_hh *)
+(*     contextual fl fr Ist r g {Rs Rt} RR my_tid ps pt nths st_src st_tgt RT (k_src: RT → itree hmodE Rs) (k_tgt: RT → itree hmodE Rt) *)
+(*     scp_src scp_tgt invspc_src invspc_tgt univ stb_src stb_tgt tid *)
+(*     (JOINS: stb_src SchName.join = Some (SchAS.join_spec univ)) *)
+(*     (JOINT: stb_tgt SchName.join = Some (SchAS.join_spec univ)) *)
+(*     : *)
+(*       ((Ist nths st_src st_tgt) ∗ *)
+(*       (∀ nths0 st_src0 st_tgt0 (ret: RT), *)
+(*         (Ist nths0 st_src0 st_tgt0) *)
+(*         -∗ @isim Σ contextual fl fr Ist my_tid r g Rs Rt RR true true nths0  *)
+(*               (st_src0, k_src ret) *)
+(*               (st_tgt0, k_tgt ret))) *)
+(*     ⊢ *)
+(*       (isim contextual fl fr Ist my_tid r g RR ps pt nths  *)
+(*         (st_src, (HMod.sandbox scp_src (interp_smod invspc_src stb_src (Sch.join RT tid)))>>= k_src) *)
+(*         (st_tgt, (HMod.sandbox scp_tgt (interp_smod invspc_tgt stb_tgt (Sch.join RT tid))) >>= k_tgt)). *)
+(*   Proof. *)
+(*     iIntros "[IST ISIM]". rewrite !/Sch.join !/ccallU. unseal "Sch". *)
+    
+(*     steps_r. inv JOINT. ss. iDestruct "GRT" as "[W PRE]". unfold precond. hss. *)
+(*     destruct q0. ss. iDestruct "PRE" as "[[% TKN] %]". des; subst; hss. *)
+
+(*     forces_l. iSplit; et. steps_l. force_l (n, o). forces_l. iSplitL "TKN W"; iFrame; et. *)
+    
+(*     call "IST"; et. *)
+
+(*     steps_l. iDestruct "ASM" as "[W [[% [% POST]] %]]". subst; hss. *)
+(*     apply SAny.downcast_upcast in G1. r in G1. subst. *)
+
+(*     forces_r. iSplitL "POST W". { iFrame; et. } *)
+(*     steps_r. hss. steps_r. rewrite SAny.upcast_downcast. hss. steps_r. *)
+(*     iApply "ISIM". iFrame. *)
+(*   Qed. *)
+
+(* End MACROAUX. *)
+
+(* Local Ltac _prep_macro_l := *)
+(*   prep; match goal with *)
+(*   | [|- context[interp_smod _ _ (Sch.spawn _ >>= _)]] => *)
+(*       rewrite// [in (interp_smod _ _ (Sch.spawn _ >>= _))] SModRed.interp_bind; _prep_macro_l *)
+(*   | [|- context[HMod.sandbox _ (interp_smod _ _ (Sch.spawn _) >>= _)]] => *)
+(*       rewrite// [in HMod.sandbox _ (interp_smod _ _ (Sch.spawn _) >>= _)] HModSB.transl_bind *)
+(*   | [|- context[interp_smod _ _ (Sch.yield >>= _)]] => *)
+(*       rewrite// [in (interp_smod _ _ (Sch.yield >>= _))] SModRed.interp_bind; _prep_macro_l *)
+(*   | [|- context[HMod.sandbox _ (interp_smod _ _ (Sch.yield) >>= _)]] => *)
+(*       rewrite// [in HMod.sandbox _ (interp_smod _ _ (Sch.yield) >>= _)] HModSB.transl_bind *)
+(*   | [|- context[interp_smod _ _ (Sch.join _ _ >>= _)]] => *)
+(*       rewrite// [in (interp_smod _ _ (Sch.join _ _ >>= _))] SModRed.interp_bind; _prep_macro_l *)
+(*   | [|- context[HMod.sandbox _ (interp_smod _ _ (Sch.join _ _) >>= _)]] => *)
+(*       rewrite// [in HMod.sandbox _ (interp_smod _ _ (Sch.join _ _) >>= _)] HModSB.transl_bind *)
+(*   end; prep. *)
+
+(* Local Ltac _prep_macro_r := *)
+(*   prep; match goal with *)
+(*   | [|- context[PMod.interp (Sch.spawn _ >>= _)]] => *)
+(*       rewrite// [in (PMod.interp (Sch.spawn _ >>= _))] PModRed.interp_bind; _prep_macro_r *)
+(*   | [|- context[HMod.sandbox _ (PMod.interp (Sch.spawn _) >>= _)]] => *)
+(*       rewrite// [in HMod.sandbox _ (PMod.interp (Sch.spawn _) >>= _)] HModSB.transl_bind *)
+(*   | [|- context[PMod.interp (Sch.yield >>= _)]] => *)
+(*       rewrite// [in (PMod.interp (Sch.yield >>= _))] PModRed.interp_bind; _prep_macro_r *)
+(*   | [|- context[HMod.sandbox _ (PMod.interp (Sch.yield) >>= _)]] => *)
+(*       rewrite// [in HMod.sandbox _ (PMod.interp (Sch.yield) >>= _)] HModSB.transl_bind *)
+(*   | [|- context[PMod.interp (Sch.join _ _ >>= _)]] => *)
+(*       rewrite// [in (PMod.interp (Sch.join _ _ >>= _))] PModRed.interp_bind; _prep_macro_r *)
+(*   | [|- context[HMod.sandbox _ (PMod.interp (Sch.join _ _) >>= _)]] => *)
+(*       rewrite// [in HMod.sandbox _ (PMod.interp (Sch.join _ _) >>= _)] HModSB.transl_bind *)
+(*   end; prep. *)
+
+(* Local Ltac prep_macro := *)
+(*   let marker := fresh "MARKER" in *)
+(*   hide_itree_r marker; try _prep_macro_l; show_itree marker; *)
+(*   hide_itree_l marker; try _prep_macro_r; show_itree marker. *)
+
+(* Ltac yield_r hyps := *)
+(*   prep_macro; *)
+(*   first [ *)
+(*     iApply isim_myield_tgt_hp; des_pairs; s; *)
+(*     [|iSplitL hyps; [|iIntros "% % %"; iIntros "[IST W]"]] | *)
+(*     iApply isim_myield_tgt_hh; des_pairs; s; *)
+(*     [|iSplitL hyps; [|iIntros "% % %"; iIntros "IST"]]]. *)
+
+(* Ltac yield_l hyps := *)
+(*   prep_macro; *)
+(*   iApply isim_myield_src; des_pairs; s; *)
+(*   [|iSplitL hyps; [ |iIntros "% % %"; iIntros "[IST W]"]]. *)
+
+(* Ltac spawn hyps := *)
+(*   prep_macro; *)
+(*   first [ *)
+(*     iApply isim_mspawn_hp; des_pairs; s; *)
+(*     [| | |iSplitL hyps; [|iIntros "% % % %"; iIntros "[IST [W TKN]]"]] | *)
+(*     iApply isim_mspawn_hh; des_pairs; s; *)
+(*     [| | |iSplitL hyps; [|iIntros "% % % %"; iIntros "IST"]]]. *)
+
+(* Ltac join hyps := *)
+(*   prep_macro; *)
+(*   first [ *)
+(*     iApply isim_mjoin_hp; des_pairs; s; *)
+(*     [|iSplitL hyps; [|iIntros "% % % %"; iIntros "[IST [W POST]]"]] | *)
+(*     iApply isim_mjoin_hh; des_pairs; s; *)
+(*     [| |iSplitL hyps; [|iIntros "% % % %"; iIntros "IST"]]]. *)
