examples/incr/IncrMainIAproof.v
@@ -1,6 +1,6 @@
 Require Import CRIS.
 
-Require Import IncrMainI IncrMainA SchA MemA wsim_tactics wsim_sch.
+Require Import IncrMainI IncrMainA SchA MemA wsim_tactics SchTactics.
 From iris Require Import frac_auth numbers.
 
 Module IncrIA. Section IncrIA.
@@ -11,14 +11,14 @@ Module IncrIA. Section IncrIA.
 
   Definition Ist : nat → alist key Any.t → alist key Any.t → iProp Σ := λ _ _ _, emp%I.
 
-  Context (u_s u_t : univ_id).
-  Context (ginv_s : invspec) (spc_s spc_user_s spc_mem : string → option fspec).
+  Context (u_s: univ_id).
+  Context (spc_s spc_user_s spc_mem : string → option fspec).
   Context (SchInSpc : spc_incl (SchAS.spc u_s spc_user_s) spc_s).
   Context (MemInSpc : spc_incl MemA.Spc spc_s).
   Context (MainInSpc : spc_incl (IncrMainAS.spc u_s) spc_user_s).
 
-  Local Notation MemA := (MemA.t ginv_s spc_mem).
-  Local Notation IncrMainA := (IncrMainA.t u_s ginv_s spc_s).
+  Local Notation MemA := (MemA.t u_s spc_mem).
+  Local Notation IncrMainA := (IncrMainA.t u_s spc_s).
   Local Notation IncrMainI := (IncrMainI.t).
   Local Notation IstFull := (IstProd (IstSB IncrMainA.(HMod.scopes) Ist) IstEq).
   Local Notation MA := (IncrMainA ★ MemA).
@@ -26,17 +26,15 @@ Module IncrIA. Section IncrIA.
 
   Lemma f_simF : HSim.sim_fun open MA MI IstFull MainName.f.
   Proof.
-    init_wsim u_s u_t.
+    winit_simF u_s 0.
 
-    w_steps_l. iDestruct "ASM" as "[[-> [C I]] ->]". hss.
+    wsteps_l. iDestruct "ASM" as "[[-> [C I]] ->]". hss.
 
-    w_step_l. rewrite SAny.upcast_downcast. hss. w_steps_l.
-
-    w_steps_r. rewrite SAny.upcast_downcast. hss. w_steps_r.
-    rewrite /IncrMainI.f /IncrMainA.f /=. w_steps_l. w_steps_r.
-  
-    _prep_macro_r. _prep_macro_l.
-    iApply (wsim_yield_tgt); first done.
+    wsteps_l. rewrite SAny.upcast_downcast. hss. wsteps_l.
+    wsteps_r. rewrite SAny.upcast_downcast. hss. wsteps_r.
+    rewrite /IncrMainI.f /IncrMainA.f /=. wsteps_l. wsteps_r.
+    
+    sch_yield_r.
     iSplitL "IST"; iFrame.
     clear nths. iIntros (nths st_s st_t) "IST".
 
@@ -44,130 +42,126 @@ Module IncrIA. Section IncrIA.
     iInv "I" as "I" "IA". SL_red.
     iDestruct "I" as (x) "PT"; SL_red; iDestruct "PT" as "[PT CA]".
 
-    w_inline_r. w_steps_r.
-    w_force_r (q5, q6, Vint x, 1%Qp).
-    w_steps_r. w_force_r ([Vptr q5 q6]↑).
-    w_steps_r. w_force_r.
+    winline_r. wsteps_r.
+    wforce_r (q5, q6, Vint x, 1%Qp).
+    wsteps_r. wforce_r ([Vptr q5 q6]↑).
+    wsteps_r. wforce_r.
     iSplitL "PT".
     { iFrame; ss. }
-    w_steps_r.
+    wsteps_r.
     iDestruct "GRT" as "[[PT ->] ->]". hss.
-    w_steps_r.
+    wsteps_r.
 
-    w_inline_r. w_steps_r.
-    w_force_r (q5, q6, Vint (x + 1)). w_steps_r.
-    w_force_r ([Vptr q5 q6; Vint (x + 1)]↑). w_steps_r.
-    w_force_r. iSplitL "PT"; iFrame; ss. w_steps_r.
-    iDestruct "GRT" as "[[PT ->] ->]". hss. w_steps_r.
+    winline_r. wsteps_r.
+    wforce_r (q5, q6, Vint (x + 1)). wsteps_r.
+    wforce_r ([Vptr q5 q6; Vint (x + 1)]↑). wsteps_r.
+    wforce_r. iSplitL "PT"; iFrame; ss. wsteps_r.
+    iDestruct "GRT" as "[[PT ->] ->]". hss. wsteps_r.
 
-    iApply wsim_yield_src; eauto.
+    sch_yield_l.
     iMod (counter_incr 1 with "[C CA]") as "[C CA]"; first iFrame.
     iMod ("IA" with "[PT CA]") as "_".
     { iExists (x + 1)%Z; SL_red; ss; iFrame. }
 
-    w_steps_l. w_force_l. w_steps_l. w_force_l. iSplitL "C"; iFrame; eauto.
-    w_steps_l. w_step; eauto.
+    wsteps_l. wforce_l. wsteps_l. wforce_l. iSplitL "C"; iFrame; eauto.
+    wsteps_l. wstep; eauto.
   Qed.
 
   Lemma main_simF : HSim.sim_fun open MA MI IstFull MainName.main.
   Proof.
-    init_wsim u_s u_t.
+    winit_simF u_s 0.
 
-    w_steps_l. iDestruct "ASM" as "[-> ->]". hss.
-    w_steps_l. _prep_macro_l.
+    wsteps_l. iDestruct "ASM" as "[-> ->]". hss.
+    wsteps_l.
 
     (* src/tgt yield *)
-    w_steps_r. _prep_macro_r.
-    iApply (wsim_yield_tgt); first done.
+    wsteps_r.
+    sch_yield_r.
     iSplitL "IST"; iFrame.
     clear nths. iIntros (nths st_s st_t) "IST".
-    iApply wsim_yield_src; first done.
+    sch_yield_l.
 
     (* src/tgt alloc *)
-    w_steps_l. w_force_l 1. w_steps_l. w_force_l. w_steps_l.
-    w_force_l. iSplit; eauto. w_steps_l.
-    w_steps_r. w_call "IST".
-    w_steps_l. iDestruct "ASM" as "[[%b [-> [PT _]]] ->]". hss. _prep_macro_l.
-    w_steps_r. hss. w_steps_r. _prep_macro_r.
+    wsteps_l. wforce_l 1. wsteps_l. wforce_l. wsteps_l.
+    wforce_l. iSplit; eauto. wsteps_l.
+    wsteps_r. wcall "IST".
+    wsteps_l. iDestruct "ASM" as "[[%b [-> [PT _]]] ->]". hss.
+    wsteps_r. hss. wsteps_r.
 
     (* tgt yield *)
-    iApply wsim_yield_tgt; first done. iFrame.
+    sch_yield_r. iFrame.
     clear nths st_s st_t. iIntros (nths st_s st_t) "IST".
 
     (* tgt store *)
-    w_inline_r. w_steps_r. w_force_r (b, 0%Z, Vint 0%Z). w_steps_r.
-    w_force_r. w_steps_r. w_force_r. iSplitL "PT".
+    winline_r. wsteps_r. wforce_r (b, 0%Z, Vint 0%Z). wsteps_r.
+    wforce_r. wsteps_r. wforce_r. iSplitL "PT".
     { iFrame. eauto. }
-    w_steps_r. iDestruct "GRT" as "[[PT ->] ->]". hss. w_steps_r. _prep_macro_r.
+    wsteps_r. iDestruct "GRT" as "[[PT ->] ->]". hss. wsteps_r.
 
     (* src/tgt yield *)
-    iApply wsim_yield_tgt; first done. iFrame.
+    sch_yield_r. iFrame.
     clear nths st_s st_t. iIntros (nths st_s st_t) "IST".
-    iApply wsim_yield_src; first done. _prep_macro_l. _prep_macro_r.
+    sch_yield_l.
 
     iApply (wsim_own_alloc (●F 0%Z ⋅ ◯F{1} 0%Z)).
     { apply frac_auth_valid; ss. }
 
     iIntros "[%γc [A F]]".
-    iMod (inv_alloc (ccounter 0 γc b 0%Z) _ _ _ N_main with "[PT A]") as "#I"; eauto.
-    { rewrite /ccounter; SL_red; iExists 0; SL_red; iFrame. }
+    iMod (inv_alloc (ccounter_syn 0 γc b 0%Z) _ _ _ N_main with "[PT A]") as "#I"; eauto.
+    { rewrite /ccounter_syn; SL_red; iExists 0; SL_red; iFrame. }
     iPoseProof (counter_op with "[F]") as "[F1 F2]".
     { rewrite -Qp.half_half -{2}(Z.add_0_r 0%Z). iApply "F". }
 
     iCombine "F1 I" as "F1". iCombine "F2 I" as "F2".
 
     (* src/tgt spawns *)
-    iApply (wsim_spawn with "IST F1").
-    { done. }
+    sch_spawn.
     { apply MainInSpc; ss. }
-    { Unshelve. 2:{ ss. exact (b, 0%Z, 0%Z, γc). }
-      2:{ exact (λ _, existT 0 (<own> γc (frac_auth_frag (1/2)%Qp 1%Z)))%SRF. }
-      { intros tid. split; ss.
-        { iIntros "[$ [C #I]]"; rewrite /precond /fspec_simple; ss; iFrame; eauto. }
-        { iIntros (ret) "[%vret [$ [[-> P] ->]]]"; ss. iExists _; iSplit; SL_red; eauto. }
-      }
+    { instantiate (1:= λ _, existT 0 (counter_syn γc (1/2)%Qp 1%Z)).
+      instantiate (2:= (b, 0%Z, 0%Z, γc)).
+      split.
+      - rewrite /precond /fspec_simple; ss.
+      - iIntros (ret) "[%vret [$ [[-> P] ->]]]"; ss.
+        iExists _; iSplit; SL_red; eauto.
     }
+    iFrame. iSplitL "" ; eauto.
     clear nths st_s st_t.
     iIntros (tid nths st_s st_t) "IST TOKEN".
-    _prep_macro_l. _prep_macro_r.
 
     (* src/tgt yield *)
-    iApply wsim_yield_tgt; first done. iFrame.
+    sch_yield_r. iFrame.
     clear nths st_s st_t. iIntros (nths st_s st_t) "IST".
-    iApply wsim_yield_src; first done. _prep_macro_l. _prep_macro_r.
+    sch_yield_l.
 
-    iApply (wsim_spawn with "IST F2").
-    { done. }
+    sch_spawn.
     { apply MainInSpc; ss. }
-    { Unshelve. 2:{ ss. exact (b, 0%Z, 0%Z, γc). }
-      2:{ exact (λ _, existT 0 (<own> γc (frac_auth_frag (1/2)%Qp 1%Z)))%SRF. }
-      { intros tid'. split; ss.
-        { iIntros "[$ [C #I]]"; rewrite /precond /fspec_simple; ss; iFrame; eauto. }
-        { iIntros (ret) "[%vret [$ [[-> P] ->]]]"; ss. iExists _; iSplit; SL_red; eauto. }
-      }
+    { instantiate (1:= λ _, existT 0 (counter_syn γc (1/2)%Qp 1%Z)).
+      instantiate (2:= (b, 0%Z, 0%Z, γc)).
+      split.
+      - rewrite /precond /fspec_simple; ss.
+      - iIntros (ret) "[%vret [$ [[-> P] ->]]]"; ss.
+        iExists _; iSplit; SL_red; eauto.
     }
+    iFrame. iSplitL "" ; eauto.
     clear nths st_s st_t.
     iIntros (tid2 nths st_s st_t) "IST TOKEN2".
-    _prep_macro_l. _prep_macro_r.
 
     (* src/tgt yield *)
-    iApply wsim_yield_tgt; first done. iFrame.
+    sch_yield_r. iFrame.
     clear nths st_s st_t. iIntros (nths st_s st_t) "IST".
-    iApply wsim_yield_src; first done. _prep_macro_l. _prep_macro_r.
+    sch_yield_l.
 
-    iApply (wsim_join with "IST TOKEN"); first done.
+    sch_join. iFrame.
     clear nths st_s st_t. iIntros (nths st_s st_t []) "IST Q /="; SL_red.
-    _prep_macro_l. _prep_macro_r.
 
-    iApply wsim_yield_tgt; first done. iFrame.
+    sch_yield_r. iFrame.
     clear nths st_s st_t. iIntros (nths st_s st_t) "IST".
-    iApply wsim_yield_src; first done. _prep_macro_l. _prep_macro_r.
+    sch_yield_l.
 
-    iApply (wsim_join with "IST TOKEN2"); first done.
+    sch_join. iFrame.
     clear nths st_s st_t. iIntros (nths st_s st_t []) "IST Q2 /="; SL_red.
-    _prep_macro_l. _prep_macro_r.
 
-    iApply wsim_yield_tgt; first done. iFrame.
+    sch_yield_r. iFrame.
     clear nths st_s st_t. iIntros (nths st_s st_t) "IST".
 
     iInv "I" as "INV" "INVA"; iEval (SL_red) in "INV"; iDestruct "INV" as "[%x INV]".
@@ -175,21 +169,21 @@ Module IncrIA. Section IncrIA.
     iCombine "C Q Q2" as "C" gives %[_ WF%frac_auth_agree]. inv WF; ss.
     iDestruct "C" as "[CA CF]".
 
-    w_inline_r. w_steps_r. w_force_r (b, 0%Z, (Vint 2), 1%Qp). w_steps_r. w_forces_r.
+    winline_r. wsteps_r. wforce_r (b, 0%Z, (Vint 2), 1%Qp). wsteps_r. wforces_r.
     iSplitL "PT"; eauto.
-    w_steps_r. iDestruct "GRT" as "[[PT ->] ->]". hss. w_steps_r. _prep_macro_r.
+    wsteps_r. iDestruct "GRT" as "[[PT ->] ->]". hss. wsteps_r.
 
     iMod ("INVA" with "[CA PT]") as "_".
     { SL_red. iExists 2; SL_red; iFrame. }
 
-    iApply wsim_yield_tgt; first done. iFrame.
+    sch_yield_r. iFrame.
     clear nths st_s st_t. iIntros (nths st_s st_t) "IST".
-    iApply wsim_yield_src; first done.
+    sch_yield_l.
 
-    w_step. w_steps_l. w_force_l. w_step_l. w_force_l. iSplit; eauto. w_steps_l.
-    w_steps_r.
+    wstep. wsteps_l. wforce_l. wstep_l. wforce_l. iSplit; eauto. wsteps_l.
+    wsteps_r.
 
-    w_step. eauto.
+    wstep. eauto.
   Qed.
 
   Lemma sim : HSim.t open MA MI emp%I IstFull.
@@ -208,12 +202,12 @@ Section wctxr.
   Context `{!SchAGΣ Σ, !memGΓ Γ, !IncrMainAGΓ Γ}.
   (* Context (I A : univ_id → HMod.modc). *)
   (* Goal <[u CTX v]= (I u) (A u). *)
-  Definition wctxr (gi : univ_id → invspec) (spc_s spc_user_s spc_mem : univ_id → string → option fspec)
+  Definition wctxr (spc_s spc_user_s spc_mem : univ_id → string → option fspec)
       (SchInSpc : ∀ u, spc_incl (SchAS.spc u (spc_user_s u)) (spc_s u))
       (MainInSpc : ∀ u, spc_incl (IncrMainAS.spc u) (spc_user_s u))
       (MemInSpc : ∀ u, spc_incl MemA.Spc (spc_s u)) :
     <[u CTX v]=
-        ((IncrMainA.t u (gi u) (spc_s u)) ★ (MemA.t (gi u) (spc_mem u)), emp%I)
-        ((IncrMainI.t)                    ★ (MemA.t (gi u) (spc_mem u)), emp%I).
+        ((IncrMainA.t u (spc_s u)) ★ (MemA.t u (spc_mem u)), emp%I)
+        ((IncrMainI.t)             ★ (MemA.t u (spc_mem u)), emp%I).
   Proof. exists 1; intros u v GE; eapply main_adequacy, sim; eauto. Defined.
 End wctxr. End IncrIA.
