theories/simulations/isim/ITacticsCommon.v
@@ -1,0 +1,816 @@
+Require Import Common.
+Require Import LAuto.
+
+Require Import Spc Mod SMod HMod PMod.
+Require Import HPSim ISimCore.
+
+(************ User Tactics **************)
+
+Ltac cong f :=
+  refine (f_equal f _).
+
+Lemma string_app_inv
+  p s s'
+  (EQ: (p ++ s = p ++ s')%string)
+  :
+  (s = s')%string.
+Proof.
+  revert_until p. induction p; i; ss.
+  unfold append in EQ. depdes EQ. eauto.
+Qed.
+
+Ltac inv_string X :=
+  inv X;
+  (hrepeat do 1 match goal with [H: @eq string _ _|-_] =>
+           apply string_app_inv in H
+     end);
+  ss.
+
+Ltac prove_scope :=
+  try unfold HMod.fnsems; try unfold SMod.fnsems; try unfold fnsems_scopes;
+  s; ii; des_ifs; ss; des; ss; eauto.
+
+Ltac prove_nodup :=
+  (hrepeat do 1 (econs; [ii; ss; des; try match goal with [H: _ |- _] => inv_string H end|]));
+  try (econs; fail).
+
+Ltac combine_quant tm :=
+  revert tm; first [apply combine_quant | apply combine_quant_dep].
+
+Definition CRIS := "cris".
+Global Opaque CRIS.
+
+Ltac unfold_hmod :=
+  match goal with
+  | [|-context[?x]] => 
+    match type of x with HMod.t =>
+      rewrite {1}/x; try unseal CRIS
+    end
+  end.
+
+Lemma ereplace T (x y: T):
+  x = y -> x = y.
+Proof. eauto. Qed.
+
+Ltac alist_upd_simpl :=
+  match goal with
+  [ |- context[alist_upd ?k ?v ?l]] =>
+    match l with
+    | context[(k,?v0)] =>
+      let TMP := fresh "_TMP" in
+      let NODUP := fresh "NODUP" in
+      match goal with [H: List.NoDup _|-_] =>
+        eassert (TMP: List.NoDup (List.map fst l)) by (exact H); clear H; revert TMP
+      end;
+      erewrite (@ereplace _ l); [intros ?|Lauto_prepare; Lauto_find (k,v0); refl];
+      eassert (NODUP := alist_upd_nodup k v _ TMP); revert NODUP;
+      rewrite !alist_upd_with_nodup; [|exact TMP]; clear TMP;
+      Lauto_finish; intros ?
+    end
+  end.
+
+Ltac move_aux :=
+  (hrepeat do 1 match goal with [H: List.NoDup _ |- _ ] => guardH H; move H at top end);
+  (hrepeat do 1 match goal with [H: Ist_monotone _ |- _ ] => guardH H; move H at top end);
+  (hrepeat do 1 match goal with [H: incl _ (HMod.scopes _ _) |- _] => guardH H; move H at top end);
+  (hrepeat do 1 match goal with [H: HMod.wf _ |- _ ] => guardH H; move H at top end);
+  (hrepeat do 1 match goal with [H: ∀ _, spc_incl _ _ |- _ ] => guardH H; move H at top end);
+  (hrepeat do 1 match goal with [H:=_:list (_ * (Any.t -> itree hmodE Any.t)) |- _ ] => guardH H; move H at top end);
+  unguard.
+
+Lemma fst_map_snd {A B C} f:
+  (fst ∘ @map_snd A B C f) = fst.
+Proof.
+  extensionalities. destruct H. s. eauto.
+Qed.
+
+Ltac fnsems_nodup H :=
+  revert H; simpl HMod.fnsems; (hrepeat do 1 unfold_hmod); simpl List.map;
+  try rewrite !List.map_map; try rewrite !fst_map_snd; eauto; fail.
+
+Ltac _alist_find_simpl :=
+  match goal with
+  [ |- context[alist_find ?k ?l]] =>
+    let TMP := fresh "_TMP" in
+    match goal with [H: List.NoDup _|-_] =>
+      eassert (TMP: List.NoDup (List.map fst l))  by (fnsems_nodup H);
+      revert TMP
+    end;
+    erewrite (@ereplace _ l); [intros ?
+    | Lauto_normalize; try rewrite !List.map_app; simpl List.map; Lauto_prepare;
+      match goal with [|-context[(?k',?v)]] => change k' with k; Lauto_find (k,v) end; refl];
+    rewrite !alist_find_with_nodup; [|exact TMP]; clear TMP;
+    Lauto_finish
+  end.
+
+Tactic Notation "alist_find_simpl_with" tactic(simpl_tac) :=
+  let GOAL := fresh "GOAL" in
+  match goal with [|-context [alist_find ?n ?x]] =>
+    pattern (alist_find n x) at 1;
+    match goal with [|- ?G _] => set (GOAL := G) end
+  end;
+  simpl HMod.fnsems; (hrepeat do 1 unfold_hmod; simpl HMod.fnsems);
+  simpl_tac;
+  unfold GOAL; clear GOAL.
+
+Ltac alist_find_simpl := alist_find_simpl_with (do 1 _alist_find_simpl).
+
+Ltac hss_des :=
+  ss; des_safe; subst;
+  (hrepeat do 1 match goal with
+    | [v: () |- _] => destruct v
+    | [H: (_,_) = (_,_) |- _] => inv H
+    end);
+  ss.
+
+Ltac hss :=
+  hss_des;
+  try (rewrite -> !Any.pair_split in * );
+  try (rewrite -> !Any.upcast_downcast in * );
+  (hrepeat do 1 match goal with [G: Any.downcast _ = Some _ |-_] =>
+    apply Any.downcast_upcast in G; inv G; ss
+   end);
+  (hrepeat do 1 match goal with [G: Any.upcast _ = Any.upcast _ |-_] =>
+    apply Any.upcast_inj in G; destruct G as [_ G]; red in G; depdes G; ss
+   end);
+  (hrepeat do 1 match goal with [G: Some _ = Some _ |- _] =>
+    depdes G; ss
+  end);
+  try (rewrite -> !Any.pair_split in * );
+  try (rewrite -> !Any.upcast_downcast in * );
+  (hrepeat do 1 alist_upd_simpl);
+  hss_des;
+  move_aux.
+
+(*** head normalization tactic ***)
+(*
+  itree term        t
+  ktree term        k
+  stuck term        s ::= opaque term
+                        | s >>= k
+                        | ↥ s
+                        | ↧ s
+                        | ░ s
+  head normal term  v ::= Ret x
+                        | Tau t
+                        | vis e k
+                        | assumeK P t
+                        | guaranteeK P t
+                        | unwrapUK x k
+                        | unwrapNK x k
+                        | HModSB.putSB scopes k v t
+                        | HModSB.getSB scopes k k
+                        | s
+ *)
+
+Inductive _hprogress := _hprogress_intro.
+
+Ltac _hprogress prg :=
+  try instantiate (1:= _hprogress_intro) in (value of prg).
+
+Ltac _hprogress_check prg :=
+  try (instantiate (1:= _hprogress_intro) in (value of prg); fail 1).
+
+Tactic Notation "red_bind" hyp(prg) tactic(tac) :=
+  lazymatch goal with
+  | [ |- @ITree.bind _ _ _ ?itr _ = _ ] =>
+      lazymatch itr with
+      | Ret _ => _hprogress prg; etransitivity; [ eapply bind_ret_l | s; tac ]
+      | Tau _ => _hprogress prg; eapply bind_tau
+      | vis _ _ => _hprogress prg; eapply vis_bind
+      | assumeK _ _ => eapply assumeK_bind
+      | guaranteeK _ _ => eapply guaranteeK_bind
+      | unwrapUK _ _ => eapply unwrapUK_bind
+      | unwrapNK _ _ => eapply unwrapNK_bind
+      | HModSB.putSB _ _ _ _ => eapply HModSB.putSB_bind
+      | HModSB.getSB _ _ _ => eapply HModSB.getSB_bind
+      | _ => reflexivity
+      end
+  end.
+
+Tactic Notation "red_SB" hyp(prg) :=
+  lazymatch goal with
+  | [ |- @HMod.sandbox _ _ _ ?itr = _ ] =>
+      lazymatch itr with
+      | Ret _ =>
+          _hprogress prg; eapply HModSB.transl_ret
+      | Tau _ =>
+          _hprogress prg; eapply HModSB.transl_tau
+      | vis (Assume _) _ =>
+          _hprogress prg; eapply HModSB.transl_vis_ag
+      | vis (Guarantee _) _ =>
+          _hprogress prg; eapply HModSB.transl_vis_ag
+      | vis (Spawn _ _) _ =>
+          _hprogress prg; eapply HModSB.transl_vis_sch
+      | vis (Yield _) _ =>
+          _hprogress prg; eapply HModSB.transl_vis_sch
+      | vis (Call _ _) _ =>
+          _hprogress prg; eapply HModSB.transl_vis_call
+      | vis (SPut _ _) _ =>
+          _hprogress prg; eapply HModSB.SPut_putSB
+      | vis (SGet _) _ =>
+          _hprogress prg; eapply HModSB.SGet_getSB
+      | vis (Choose _) _ =>
+          _hprogress prg; eapply HModSB.transl_vis_core
+      | vis (Take _) _ =>
+          _hprogress prg; eapply HModSB.transl_vis_core
+      | vis (IO _ _) _ =>
+          _hprogress prg; eapply HModSB.transl_vis_core
+      | assumeK _ _ =>
+          _hprogress prg; eapply HModSB.transl_assumeK
+      | guaranteeK _ _ =>
+          _hprogress prg; eapply HModSB.transl_guaranteeK
+      | unwrapUK _ _ =>
+          _hprogress prg; eapply HModSB.transl_unwrapUK
+      | unwrapNK _ _ =>
+          _hprogress prg; eapply HModSB.transl_unwrapNK
+      | _ =>
+          reflexivity
+      end
+  end.
+
+Ltac unfold_spc_exact spc name :=
+  try match goal with
+      [ H : spc_incl _ spc |- _ ] =>
+        let RW := fresh "_RW" in
+        let ND := fresh "_ND" in
+        edestruct H as [ND RW];
+        erewrite (RW name);
+        [| revert ND; unfold to_spc;
+           match goal with [|-context[alist_find _ ?x]] => rewrite /x end;
+           unseal CRIS; i;
+           alist_find_simpl;
+           refl];
+        simpl unwrapN; clear ND RW
+    end.
+
+Tactic Notation "red_S" hyp(prg) tactic(tac) :=
+  lazymatch goal with
+  | [ |- @interp_smod ?Σ ?ginv ?stb ?R ?itr = _ ] =>
+      lazymatch itr with
+      | Ret _ =>
+          _hprogress prg; eapply SModRed.interp_ret
+      | Tau _ =>
+          _hprogress prg; eapply SModRed.interp_tau
+      | vis (Assume _) _ =>
+          _hprogress prg; eapply SModRed.interp_vis_ag
+      | vis (Guarantee _) _ =>
+          _hprogress prg; eapply SModRed.interp_vis_ag
+      | vis (Spawn _ _) _ =>
+          _hprogress prg; etransitivity;
+          [ eapply SModRed.interp_vis_sch
+          | unfold handle_schE_hmodE;
+            unfold HoareSpawn;
+            tac
+          ]
+      | vis (Yield _) _ =>
+          _hprogress prg; etransitivity;
+          [ eapply SModRed.interp_vis_sch
+          | unfold handle_schE_hmodE;
+            unfold HoareYield;
+            tac
+          ]
+      | vis (Call ?fn _) _ =>
+          _hprogress prg; etransitivity;
+          [ eapply SModRed.interp_vis_call
+          | unfold handle_callE_hmodE;
+            unfold HoareCall;
+            unfold_spc_exact stb fn;
+            tac
+          ]
+      | vis (SPut _ _) _ =>
+          _hprogress prg; eapply SModRed.interp_vis_pg
+      | vis (SGet _) _ =>
+          _hprogress prg; eapply SModRed.interp_vis_pg
+      | vis (Choose _) _ =>
+          _hprogress prg; eapply SModRed.interp_vis_core
+      | vis (Take _) _ =>
+          _hprogress prg; eapply SModRed.interp_vis_core
+      | vis (IO _ _) _ =>
+          _hprogress prg; eapply SModRed.interp_vis_core
+      | assumeK _ _ =>
+          _hprogress prg; eapply SModRed.interp_assumeK
+      | guaranteeK _ _ =>
+          _hprogress prg; eapply SModRed.interp_guaranteeK
+      | unwrapUK _ _ =>
+          _hprogress prg; eapply SModRed.interp_unwrapUK
+      | unwrapNK _ _ =>
+          _hprogress prg; eapply SModRed.interp_unwrapNK
+      | _ =>
+          reflexivity
+      end
+  end.
+
+Tactic Notation "red_P" hyp(prg) :=
+  lazymatch goal with
+  | [ |- @PMod.interp _ _ ?itr = _ ] =>
+      lazymatch itr with
+      | Ret _ =>
+          _hprogress prg; eapply PModRed.interp_ret
+      | Tau _ =>
+          _hprogress prg; eapply PModRed.interp_tau
+      | vis (Spawn _ _) _ =>
+          _hprogress prg; eapply PModRed.interp_vis_sch
+      | vis (Yield _) _ =>
+          _hprogress prg; eapply PModRed.interp_vis_sch
+      | vis (Call _ _) _ =>
+          _hprogress prg; eapply PModRed.interp_vis_call
+      | vis (SPut _ _) _ =>
+          _hprogress prg; eapply PModRed.interp_vis_pg
+      | vis (SGet _) _ =>
+          _hprogress prg; eapply PModRed.interp_vis_pg
+      | vis (Choose _) _ =>
+          _hprogress prg; eapply PModRed.interp_vis_choose
+      | vis (Take _) _ =>
+          _hprogress prg; eapply PModRed.interp_vis_take
+      | vis (IO _ _) _ =>
+          _hprogress prg; eapply PModRed.interp_vis_io
+      | assumeK _ _ =>
+          _hprogress prg; eapply PModRed.interp_assumeK
+      | guaranteeK _ _ =>
+          _hprogress prg; eapply PModRed.interp_guaranteeK
+      | unwrapUK _ _ =>
+          _hprogress prg; eapply PModRed.interp_unwrapUK
+      | unwrapNK _ _ =>
+          _hprogress prg; eapply PModRed.interp_unwrapNK
+      | _ =>
+          reflexivity
+      end
+  end.
+
+Ltac _hnorm_itr prg :=
+  lazymatch goal with
+  | [ |- Ret _ = _ ] =>
+      reflexivity
+  | [ |- Tau _ = _ ] =>
+      reflexivity
+  | [ |- vis _ _ = _ ] =>
+      reflexivity
+  | [ |- @ITree.bind ?E ?T ?U ?itr ?ktr = _ ] =>
+      etransitivity;
+      [ let itr' := fresh "itr" in cong (fun itr' => @ITree.bind E T U itr' ktr); _hnorm_itr prg | red_bind prg (do 1 _hnorm_itr prg) ]
+  | [ |- @HMod.sandbox ?Σ ?R ?scopes ?itr = _ ] =>
+      etransitivity;
+      [ cong (@HMod.sandbox Σ R scopes); _hnorm_itr prg | red_SB prg ]
+  | [ |- @interp_smod ?Σ ?ginv ?stb ?R ?itr = _ ] =>
+      etransitivity;
+      [ cong (@interp_smod Σ ginv stb R); _hnorm_itr prg | red_S prg (do 1 _hnorm_itr prg) ]
+  | [ |- @PMod.interp ?Σ ?R ?itr = _ ] =>
+      etransitivity;
+      [ cong (@PMod.interp Σ R); _hnorm_itr prg | red_P prg ]
+  | [ |- trigger _ = _ ] =>
+      eapply trigger_vis
+  | [ |- assume _ = _ ] =>
+      eapply assume_assumeK
+  | [ |- guarantee _ = _ ] =>
+      eapply guarantee_guaranteeK
+  | [ |- unwrapU _ = _ ] =>
+      eapply unwrapU_unwrapUK
+  | [ |- unwrapN _ = _ ] =>
+      eapply unwrapN_unwrapNK
+  | [ |- HoareCall _ _ _ = _ ] =>
+      _hprogress prg; unfold HoareCall;
+      _hnorm_itr prg
+  | [ |- HoareSpawn _ _ _ _ = _ ] =>
+      _hprogress prg; unfold HoareSpawn;
+      _hnorm_itr prg
+  | [ |- HoareYield _ _ = _ ] =>
+      _hprogress prg; unfold HoareYield;
+      _hnorm_itr prg
+  | [ |- fbody_trivial _ = _ ] =>
+      _hprogress prg; unfold fbody_trivial;
+      _hnorm_itr prg
+  | [ |- cput _ _ = _ ] =>
+      _hprogress prg; unfold cput;
+      _hnorm_itr prg
+  | [ |- cgetU _ = _ ] =>
+      _hprogress prg; unfold cgetU;
+      _hnorm_itr prg
+  | [ |- cgetN _ = _ ] =>
+      _hprogress prg; unfold cgetN;
+      _hnorm_itr prg
+  | [ |- cfunU _ _ = _ ] =>
+      _hprogress prg; unfold cfunU;
+      _hnorm_itr prg
+  | [ |- cfunN _ _ = _ ] =>
+      _hprogress prg; unfold cfunN;
+      _hnorm_itr prg
+  | [ |- ccallU _ _ = _ ] =>
+      _hprogress prg; unfold ccallU;
+      _hnorm_itr prg
+  | [ |- ccallN _ _ = _ ] =>
+      _hprogress prg; unfold ccallN;
+      _hnorm_itr prg
+  | [ |- triggerUB = _ ] =>
+      _hprogress prg; unfold triggerUB;
+      _hnorm_itr prg
+  | [ |- triggerNB = _ ] =>
+      _hprogress prg; unfold triggerNB;
+      _hnorm_itr prg
+  | [ |- ?itr = _ ] =>
+      reflexivity
+  end.
+
+Ltac hnorm_itr :=
+  try match goal with
+  | [ |- @ITree.bind _ _ _ (trigger _) _ = _ ] => fail 2
+  end;
+  let prg := fresh "Progress" in
+  epose (prg := _ : _hprogress);
+  etransitivity;
+  [ _hnorm_itr prg
+  | _hprogress_check prg; s;
+    lazymatch goal with
+    | [ |- Ret _ = _ ] =>
+        reflexivity
+    | [ |- Tau _ = _ ] =>
+        reflexivity
+    | [ |- vis _ _ = _ ] =>
+        eapply vis_trigger
+    | [ |- assumeK _ _ = _ ] =>
+        eapply assumeK_assume
+    | [ |- guaranteeK _ _ = _ ] =>
+        eapply guaranteeK_guarantee
+    | [ |- unwrapUK _ _ = _ ] =>
+        eapply unwrapUK_unwrapU
+    | [ |- unwrapNK _ _ = _ ] =>
+        eapply unwrapNK_unwrapN
+    | [ |- HModSB.putSB _ _ _ _ = _ ] =>
+        eapply HModSB.putSB_SPut
+    | [ |- HModSB.getSB _ _ _ = _ ] =>
+        eapply HModSB.getSB_SGet
+    | [ |- _ = _ ] =>
+        reflexivity
+    end
+  ].
+
+Ltac iIntrosFresh H := iIntros H || iIntrosFresh (H ++ "'")%string.
+
+Ltac des_pairs :=
+  (hrepeat do 1
+    match goal with
+    | [H: context[let () := ?x in _] |- _] =>
+        match type of x with
+        | () => destruct x
+        | (_ * _)%type =>
+            let n0 := fresh "q" in let n1 := fresh "q" in
+            let EQ := fresh "EQq" in
+            destruct x as [n0 n1] eqn: EQ
+        end
+    | |- context[let () := ?x in _] =>
+        match type of x with
+        | () => destruct x
+        | (_ * _)%type =>
+            let n0 := fresh "q" in let n1 := fresh "q" in
+            let EQ := fresh "EQq" in
+            destruct x as [n0 n1] eqn: EQ
+        end
+    end);
+   subst.
+
+Ltac has_precond_in TM :=
+  match goal with [H := ?P |- _] => match H with TM => match P with context[precond] => idtac end end end.
+Ltac has_postcond_in TM :=
+  match goal with [H := ?P |- _] => match H with TM => match P with context[postcond] => idtac end end end.
+Ltac unfold_precond_postcond term := let TM := fresh "_term" in
+  set (TM := term) at 1;
+  (hrepeat do 1 (has_precond_in TM; unfold precond in TM; simpl in TM));
+  (hrepeat do 1 (has_postcond_in TM; unfold postcond in TM; simpl in TM));
+  subst TM.
+
+Ltac set_marker marker :=
+  assert (marker: True) by exact I.
+
+Ltac hide_ihyps_env env :=
+  match env with
+  | environments.Enil => idtac
+  | environments.Esnoc ?tl _ ?hyp =>
+      hide_ihyps_env tl;
+      let IHYP := fresh "IHYP" in
+      set (IHYP := hyp) at 1
+  end.
+
+Ltac hide_ihyps :=
+  match goal with
+  | [ |- environments.envs_entails {|environments.env_intuitionistic := ?ienv; environments.env_spatial := ?env |} _] =>
+      hide_ihyps_env ienv;
+      hide_ihyps_env env
+  end.
+
+Ltac hide_itree_l :=
+  let ITREE := fresh "ITREE" in
+  match goal with [|- _ (_ (_, ?it) _)] => set (ITREE := it) at 1 end.
+
+Ltac hide_itree_r :=
+  let ITREE := fresh "ITREE" in
+  match goal with
+  [|- _ (_ _ (_, ?it))] => first [set (ITREE := it) at 2|set (ITREE := it) at 1]
+  end.
+
+Ltac show_itree :=
+  match goal with [H:_|-_] => unfold H; clear H end.
+
+Ltac show_until marker :=
+  (hrepeat do 1 match goal with
+      [H: _ |- _] =>
+        try match H with marker => fail 3 end;
+        first [unfold H; clear H | revert H]
+    end);
+  clear marker; i.
+
+Ltac unfold_cris_defs :=
+  (hrepeat do 1 match goal with
+  | [|- context[{| fsb_body := cfunU ?x |}]] => rewrite {1}/x
+  | [|- context[{| fsb_body := cfunN ?x |}]] => rewrite {1}/x
+  | [|- context[{| fsb_body := ?x |}]] => rewrite {1}/x
+  | [|- context[PMod.interp (?x _)]] => unfold x
+  | [|- context[cfunU ?x]] => rewrite {1}/x
+  | [|- context[cfunN ?x]] => rewrite {1}/x
+  end);
+  unfold interp_sb_hp, HoareFun, cfunU, cfunN, HMod.sandbox_body; s.  
+
+Ltac hide_flist :=
+  let FLS := fresh "FLS" in let FLT := fresh "FLT" in
+  match goal with [|- context[(isim_fsem ?fls ?flt _ _)]] =>
+    set (FLS := fls); set (FLT := flt)
+  end.
+
+Ltac pre_simF :=
+  unfold HSim.sim_fun; i;
+  match goal with [H: _|-_] => revert H end;
+  hide_flist.
+
+Ltac post_simF :=
+  eexists; split; [eauto|];
+  unfold_cris_defs;
+  ii; subst; iIntros "IST";
+  move_aux.
+
+Ltac init_simF :=
+  pre_simF;
+  alist_find_simpl;
+  let H := fresh "H" in intro H; inv H;
+  alist_find_simpl;
+  post_simF.
+
+Ltac prove_sub_perm :=  
+  i; try rewrite /HMod.scopes; s; (hrepeat do 1 unfold_hmod); s;
+  match goal with
+    [|-sub_perm ?x ?y] =>
+      match x with
+      | _ :: _ => idtac
+      | _ => try rewrite /x
+      end;
+      match y with
+      | _ :: _ => idtac
+      | _ => try rewrite /y
+      end
+  end;
+  (hrepeat do 1 s;
+   match goal with [|-sub_perm (?k::_) ?tgt] =>
+     let key := fresh "key" in
+     set (key := k);
+     match tgt with
+     |  context[?k'::_] =>
+          change k' with key;
+          eapply eq_ind; [|symmetry; Lauto_prepare; Lauto_find key; refl];
+          eapply (sub_perm_cancel [key] [])
+     end;
+     unfold key; clear key
+  end);
+  apply sub_perm_nil.
+
+Ltac prove_inline_cond :=
+  first [eassumption |
+  match goal with [|- alist_find _ ?FL = _] =>
+    rewrite /FL;
+    simpl HMod.fnsems; (hrepeat do 1 unfold_hmod);
+    simpl List.map; alist_find_simpl; eauto
+  end].
+
+Ltac unfold_iter_l :=
+  let marker := fresh "MARKER" in
+  set_marker marker;
+  hide_ihyps;
+  hide_itree_r;
+  rewrite unfold_iter_eq;
+  show_until marker.
+
+Ltac unfold_iter_r :=
+  let marker := fresh "MARKER" in
+  set_marker marker;
+  hide_ihyps;
+  hide_itree_l;
+  rewrite unfold_iter_eq;
+  show_until marker.
+
+(***
+ Rewriting-based normalization
+ ***)
+
+Ltac unfold_spc :=
+  try match goal with
+    [|-context[unwrapN (?spc ?name)]] =>
+      try match goal with
+        [H: context[spc_incl _ spc]|-_] =>
+          let RW := fresh "_RW" in let ND := fresh "_ND" in
+          edestruct H as [ND RW];
+          erewrite (RW name);
+          [|revert ND; unfold to_spc;
+            match goal with [|-context[alist_find _ ?x]] => rewrite /x end;
+            unseal CRIS; i;
+            alist_find_simpl;
+            refl];
+          simpl unwrapN; clear ND RW
+      end
+  end.
+
+Ltac desugar itr :=
+  match itr with
+  | fbody_trivial _ => rewrite {1}/itr
+  | HoareCall _ _ _ => rewrite {1}/itr
+  | HoareSpawn _ _ _ => rewrite {1}/itr
+  | HoareYield _ _ => rewrite {1}/itr
+  | cput _ _ => rewrite{1}/itr
+  | cgetU _ => rewrite{1}/itr
+  | cgetN _ => rewrite{1}/itr
+  | triggerUB => rewrite{1}/itr
+  | triggerNB => rewrite{1}/itr
+  end.
+
+Ltac _unwrapSB itr :=
+  match itr with
+  | Ret _ =>
+      rewrite HModSB.transl_ret
+  | tau;; _ =>
+      rewrite HModSB.transl_tau
+  | trigger (Choose _) =>
+      rewrite HModSB.transl_core
+  | trigger (Take _) =>
+      rewrite HModSB.transl_core
+  | trigger (IO _ _) =>
+      rewrite HModSB.transl_core
+  | trigger (Call _ _) =>
+      rewrite HModSB.transl_call
+  | trigger (SPut _ _) =>
+      idtac
+  | trigger (SGet _) =>
+      idtac
+  | trigger (Assume _) =>
+      rewrite HModSB.transl_ag
+  | trigger (Guarantee _) =>
+      rewrite HModSB.transl_ag
+  | unwrapU _ =>
+      rewrite HModSB.transl_unwrapU
+  | unwrapN _ =>
+      rewrite HModSB.transl_unwrapN
+  | assume _ =>
+      rewrite HModSB.transl_asm
+  | guarantee _ =>
+      rewrite HModSB.transl_guar
+  | trigger (Spawn _ _) =>
+      rewrite HModSB.transl_sch
+  | trigger (Yield _) =>
+      rewrite HModSB.transl_sch
+  | _ => fail
+  end.
+
+Ltac unwrapSB :=
+  try match goal with
+  | [|-context[HMod.sandbox _ ?itr]] => first [desugar itr|fail 2]
+  end;
+  match goal with
+  | [|-context[HMod.sandbox _ (?itr >>= _)]] =>
+      rewrite HModSB.transl_bind; unwrapSB
+  | [|-context[HMod.sandbox _ ?itr]] => first [_unwrapSB itr|fail 2]
+  end.
+
+Ltac _unwrapS itr :=
+  match itr with
+  | Ret _ =>
+      rewrite SModRed.interp_ret
+  | tau;; _ =>
+      rewrite SModRed.interp_tau
+  | trigger (Choose _) =>
+      rewrite SModRed.interp_core
+  | trigger (Take _) =>
+      rewrite SModRed.interp_core
+  | trigger (IO _ _) =>
+      rewrite SModRed.interp_core
+  | trigger (Call _ _) =>
+      rewrite SModRed.interp_call {1}/handle_callE_hmodE
+  | trigger (Spawn _ _) =>
+      rewrite SModRed.interp_sch {1}/handle_schE_hmodE
+  | trigger (Yield _) =>
+      rewrite SModRed.interp_sch {1}/handle_schE_hmodE
+  | trigger (SPut _ _) =>
+      rewrite SModRed.interp_pg
+  | trigger (SGet _) =>
+      rewrite SModRed.interp_pg
+  | trigger (Assume _) =>
+      rewrite SModRed.interp_ag
+  | trigger (Guarantee _) =>
+      rewrite SModRed.interp_ag
+  | unwrapU _ =>
+      rewrite SModRed.interp_unwrapU
+  | unwrapN _ =>
+      rewrite SModRed.interp_unwrapN
+  | assume _ =>
+      rewrite SModRed.interp_asm
+  | guarantee _ =>
+      rewrite SModRed.interp_guar
+  | _ => fail
+  end.
+
+Ltac unwrapS :=
+  try match goal with
+    | [|-context[interp_smod _ _ ?itr]] => first [desugar itr|fail 2]
+  end;
+  match goal with
+  | [|-context[interp_smod _ _ (?itr >>= _)]] =>
+      rewrite SModRed.interp_bind; unwrapS
+  | [|-context[interp_smod _ _ ?itr]] => first [_unwrapS itr|fail 2]
+  end.
+
+Ltac _unwrapP itr :=
+  match itr with
+  | Ret _ =>
+      rewrite PModRed.interp_ret
+  | tau;; _ =>
+      rewrite PModRed.interp_tau
+  | trigger (Choose _) =>
+      rewrite PModRed.interp_choose
+  | trigger (Take _) =>
+      rewrite PModRed.interp_take
+  | trigger (IO _ _) =>
+      rewrite PModRed.interp_io
+  | trigger (Call _ _) =>
+      rewrite PModRed.interp_call
+  | trigger (Spawn _ _) =>
+      rewrite PModRed.interp_sch
+  | trigger (Yield _) =>
+      rewrite PModRed.interp_sch
+  | trigger (SPut _ _) =>
+      rewrite PModRed.interp_pg
+  | trigger (SGet _) =>
+      rewrite PModRed.interp_pg
+  | unwrapU _ =>
+      rewrite PModRed.interp_unwrapU
+  | unwrapN _ =>
+      rewrite PModRed.interp_unwrapN
+  | assume _ =>
+      rewrite PModRed.interp_asm
+  | guarantee _ =>
+      rewrite PModRed.interp_guar
+  | _ => fail
+  end.
+
+Ltac unwrapP :=
+  try match goal with
+  | [|-context[PMod.interp ?itr]] => first [desugar itr|fail 2]
+  end;
+  match goal with
+  | [|-context[PMod.interp (?itr >>= _)]] =>
+      rewrite PModRed.interp_bind; unwrapP
+  | [|-context[PMod.interp ?itr]] => first [_unwrapP itr|fail 2]
+  end.
+
+Ltac _prep :=
+  first
+    [ unwrapSB
+    | unwrapS; unfold_spc; unwrapSB
+    | unwrapP; unwrapSB
+    | idtac].
+
+Ltac prep :=
+  try rewrite !bind_bind;
+  try match goal with
+  | [|-context[interp_smod _ _ (?f ?arg)]] =>
+    match type of arg with Any.t => rewrite {1}/f end
+  | [|-context[PMod.interp (?f ?arg)]] =>
+    match type of arg with Any.t => rewrite {1}/f end
+  end;
+  unfold ccallU, ccallN;
+  try match goal with
+      | [|-context[(_, HMod.sandbox _ _)]] => _prep
+      | [|-context[(_, HMod.sandbox _ _ >>= _)]] => _prep
+      end;
+  try rewrite !bind_bind;
+  try rewrite !bind_tau.
+
+Ltac prep_l :=
+  let marker := fresh "MARKER" in
+  set_marker marker;
+  hide_ihyps;
+  hide_itree_r;
+  prep;
+  show_until marker.
+
+Ltac prep_r :=
+  let marker := fresh "MARKER" in
+  set_marker marker;
+  hide_ihyps;
+  hide_itree_l;
+  prep;
+  show_until marker.
+
