theories/simulations/isim/ITacticsCore.v
@@ -3,1043 +3,24 @@ Require Import LAuto.
 
 Require Import Spc Mod SMod HMod PMod.
 Require Import HPSim ISimCore.
-
-(************ User Tactics **************)
-
-Ltac cong f :=
-  refine (f_equal f _).
-
-Lemma string_app_inv
-  p s s'
-  (EQ: (p ++ s = p ++ s')%string)
-  :
-  (s = s')%string.
-Proof.
-  revert_until p. induction p; i; ss.
-  unfold append in EQ. depdes EQ. eauto.
-Qed.
-
-Ltac inv_string X :=
-  inv X;
-  (hrepeat do 1 match goal with [H: @eq string _ _|-_] =>
-           apply string_app_inv in H
-     end);
-  ss.
-
-Ltac prove_scope :=
-  try unfold HMod.fnsems; try unfold SMod.fnsems; try unfold fnsems_scopes;
-  s; ii; des_ifs; ss; des; ss; eauto.
-
-Ltac prove_nodup :=
-  (hrepeat do 1 (econs; [ii; ss; des; try match goal with [H: _ |- _] => inv_string H end|]));
-  try (econs; fail).
-
-Ltac combine_quant tm :=
-  revert tm; first [apply combine_quant | apply combine_quant_dep].
-
-Ltac by_coind CIH :=
-  iApply isim_progress; iApply isim_base;
-  iSpecialize (CIH $! _);
-  (hrepeat do 1 first[instantiate (1:= (_,_))|instantiate (1:= existT _ _)]); s;
-  iApply CIH.
-
-Definition CRIS := "cris".
-Global Opaque CRIS.
-
-Ltac unfold_hmod :=
-  match goal with
-  | [|-context[?x]] => 
-    match type of x with HMod.t =>
-      rewrite {1}/x; try unseal CRIS
-    end
-  end.
-
-Lemma ereplace T (x y: T):
-  x = y -> x = y.
-Proof. eauto. Qed.
-
-Ltac alist_upd_simpl :=
-  match goal with
-  [ |- context[alist_upd ?k ?v ?l]] =>
-    match l with
-    | context[(k,?v0)] =>
-      let TMP := fresh "_TMP" in
-      let NODUP := fresh "NODUP" in
-      match goal with [H: List.NoDup _|-_] =>
-        eassert (TMP: List.NoDup (List.map fst l)) by (exact H); clear H; revert TMP
-      end;
-      erewrite (@ereplace _ l); [intros ?|Lauto_prepare; Lauto_find (k,v0); refl];
-      eassert (NODUP := alist_upd_nodup k v _ TMP); revert NODUP;
-      rewrite !alist_upd_with_nodup; [|exact TMP]; clear TMP;
-      Lauto_finish; intros ?
-    end
-  end.
-
-Ltac move_aux :=
-  (hrepeat do 1 match goal with [H: List.NoDup _ |- _ ] => guardH H; move H at top end);
-  (hrepeat do 1 match goal with [H: Ist_monotone _ |- _ ] => guardH H; move H at top end);
-  (hrepeat do 1 match goal with [H: incl _ (HMod.scopes _ _) |- _] => guardH H; move H at top end);
-  (hrepeat do 1 match goal with [H: HMod.wf _ |- _ ] => guardH H; move H at top end);
-  (hrepeat do 1 match goal with [H: ∀ _, spc_incl _ _ |- _ ] => guardH H; move H at top end);
-  (hrepeat do 1 match goal with [H:=_:list (_ * (Any.t -> itree hmodE Any.t)) |- _ ] => guardH H; move H at top end);
-  unguard.
-
-Lemma fst_map_snd {A B C} f:
-  (fst ∘ @map_snd A B C f) = fst.
-Proof.
-  extensionalities. destruct H. s. eauto.
-Qed.
-
-Ltac fnsems_nodup H :=
-  revert H; simpl HMod.fnsems; (hrepeat do 1 unfold_hmod); simpl List.map;
-  try rewrite !List.map_map; try rewrite !fst_map_snd; eauto; fail.
-
-Ltac _alist_find_simpl :=
-  match goal with
-  [ |- context[alist_find ?k ?l]] =>
-    let TMP := fresh "_TMP" in
-    match goal with [H: List.NoDup _|-_] =>
-      eassert (TMP: List.NoDup (List.map fst l))  by (fnsems_nodup H);
-      revert TMP
-    end;
-    erewrite (@ereplace _ l); [intros ?
-    | Lauto_normalize; try rewrite !List.map_app; simpl List.map; Lauto_prepare;
-      match goal with [|-context[(?k',?v)]] => change k' with k; Lauto_find (k,v) end; refl];
-    rewrite !alist_find_with_nodup; [|exact TMP]; clear TMP;
-    Lauto_finish
-  end.
-
-Tactic Notation "alist_find_simpl_with" tactic(simpl_tac) :=
-  let GOAL := fresh "GOAL" in
-  match goal with [|-context [alist_find ?n ?x]] =>
-    pattern (alist_find n x) at 1;
-    match goal with [|- ?G _] => set (GOAL := G) end
-  end;
-  simpl HMod.fnsems; (hrepeat do 1 unfold_hmod; simpl HMod.fnsems);
-  simpl_tac;
-  unfold GOAL; clear GOAL.
-
-Ltac alist_find_simpl := alist_find_simpl_with (do 1 _alist_find_simpl).
-
-Ltac hss_des :=
-  ss; des_safe; subst;
-  (hrepeat do 1 match goal with
-    | [v: () |- _] => destruct v
-    | [H: (_,_) = (_,_) |- _] => inv H
-    end);
-  ss.
-
-Ltac hss :=
-  hss_des;
-  try (rewrite -> !Any.pair_split in * );
-  try (rewrite -> !Any.upcast_downcast in * );
-  (hrepeat do 1 match goal with [G: Any.downcast _ = Some _ |-_] =>
-    apply Any.downcast_upcast in G; inv G; ss
-   end);
-  (hrepeat do 1 match goal with [G: Any.upcast _ = Any.upcast _ |-_] =>
-    apply Any.upcast_inj in G; destruct G as [_ G]; red in G; depdes G; ss
-   end);
-  (hrepeat do 1 match goal with [G: Some _ = Some _ |- _] =>
-    depdes G; ss
-  end);
-  try (rewrite -> !Any.pair_split in * );
-  try (rewrite -> !Any.upcast_downcast in * );
-  (hrepeat do 1 alist_upd_simpl);
-  hss_des;
-  move_aux.
-
-(*** head normalization tactic ***)
-(*
-  itree term        t
-  ktree term        k
-  stuck term        s ::= opaque term
-                        | s >>= k
-                        | ↥ s
-                        | ↧ s
-                        | ░ s
-  head normal term  v ::= Ret x
-                        | Tau t
-                        | vis e k
-                        | assumeK P t
-                        | guaranteeK P t
-                        | unwrapUK x k
-                        | unwrapNK x k
-                        | HModSB.putSB scopes k v t
-                        | HModSB.getSB scopes k k
-                        | s
- *)
-
-Inductive _hprogress := _hprogress_intro.
-
-Ltac _hprogress prg :=
-  try instantiate (1:= _hprogress_intro) in (value of prg).
-
-Ltac _hprogress_check prg :=
-  try (instantiate (1:= _hprogress_intro) in (value of prg); fail 1).
-
-Tactic Notation "red_bind" hyp(prg) tactic(tac) :=
-  lazymatch goal with
-  | [ |- @ITree.bind _ _ _ ?itr _ = _ ] =>
-      lazymatch itr with
-      | Ret _ => _hprogress prg; etransitivity; [ eapply bind_ret_l | s; tac ]
-      | Tau _ => _hprogress prg; eapply bind_tau
-      | vis _ _ => _hprogress prg; eapply vis_bind
-      | assumeK _ _ => eapply assumeK_bind
-      | guaranteeK _ _ => eapply guaranteeK_bind
-      | unwrapUK _ _ => eapply unwrapUK_bind
-      | unwrapNK _ _ => eapply unwrapNK_bind
-      | HModSB.putSB _ _ _ _ => eapply HModSB.putSB_bind
-      | HModSB.getSB _ _ _ => eapply HModSB.getSB_bind
-      | _ => reflexivity
-      end
-  end.
-
-Tactic Notation "red_SB" hyp(prg) :=
-  lazymatch goal with
-  | [ |- @HMod.sandbox _ _ _ ?itr = _ ] =>
-      lazymatch itr with
-      | Ret _ =>
-          _hprogress prg; eapply HModSB.transl_ret
-      | Tau _ =>
-          _hprogress prg; eapply HModSB.transl_tau
-      | vis (Assume _) _ =>
-          _hprogress prg; eapply HModSB.transl_vis_ag
-      | vis (Guarantee _) _ =>
-          _hprogress prg; eapply HModSB.transl_vis_ag
-      | vis (Spawn _ _) _ =>
-          _hprogress prg; eapply HModSB.transl_vis_sch
-      | vis (Yield _) _ =>
-          _hprogress prg; eapply HModSB.transl_vis_sch
-      | vis (Call _ _) _ =>
-          _hprogress prg; eapply HModSB.transl_vis_call
-      | vis (SPut _ _) _ =>
-          _hprogress prg; eapply HModSB.SPut_putSB
-      | vis (SGet _) _ =>
-          _hprogress prg; eapply HModSB.SGet_getSB
-      | vis (Choose _) _ =>
-          _hprogress prg; eapply HModSB.transl_vis_core
-      | vis (Take _) _ =>
-          _hprogress prg; eapply HModSB.transl_vis_core
-      | vis (IO _ _) _ =>
-          _hprogress prg; eapply HModSB.transl_vis_core
-      | assumeK _ _ =>
-          _hprogress prg; eapply HModSB.transl_assumeK
-      | guaranteeK _ _ =>
-          _hprogress prg; eapply HModSB.transl_guaranteeK
-      | unwrapUK _ _ =>
-          _hprogress prg; eapply HModSB.transl_unwrapUK
-      | unwrapNK _ _ =>
-          _hprogress prg; eapply HModSB.transl_unwrapNK
-      | _ =>
-          reflexivity
-      end
-  end.
-
-Ltac unfold_spc_exact spc name :=
-  try match goal with
-      [ H : spc_incl _ spc |- _ ] =>
-        let RW := fresh "_RW" in
-        let ND := fresh "_ND" in
-        edestruct H as [ND RW];
-        erewrite (RW name);
-        [| revert ND; unfold to_spc;
-           match goal with [|-context[alist_find _ ?x]] => rewrite /x end;
-           unseal CRIS; i;
-           alist_find_simpl;
-           refl];
-        simpl unwrapN; clear ND RW
-    end.
-
-Tactic Notation "red_S" hyp(prg) tactic(tac) :=
-  lazymatch goal with
-  | [ |- @interp_smod ?Σ ?ginv ?stb ?R ?itr = _ ] =>
-      lazymatch itr with
-      | Ret _ =>
-          _hprogress prg; eapply SModRed.interp_ret
-      | Tau _ =>
-          _hprogress prg; eapply SModRed.interp_tau
-      | vis (Assume _) _ =>
-          _hprogress prg; eapply SModRed.interp_vis_ag
-      | vis (Guarantee _) _ =>
-          _hprogress prg; eapply SModRed.interp_vis_ag
-      | vis (Spawn _ _) _ =>
-          _hprogress prg; etransitivity;
-          [ eapply SModRed.interp_vis_sch
-          | unfold handle_schE_hmodE;
-            unfold HoareSpawn;
-            tac
-          ]
-      | vis (Yield _) _ =>
-          _hprogress prg; etransitivity;
-          [ eapply SModRed.interp_vis_sch
-          | unfold handle_schE_hmodE;
-            unfold HoareYield;
-            tac
-          ]
-      | vis (Call ?fn _) _ =>
-          _hprogress prg; etransitivity;
-          [ eapply SModRed.interp_vis_call
-          | unfold handle_callE_hmodE;
-            unfold HoareCall;
-            unfold_spc_exact stb fn;
-            tac
-          ]
-      | vis (SPut _ _) _ =>
-          _hprogress prg; eapply SModRed.interp_vis_pg
-      | vis (SGet _) _ =>
-          _hprogress prg; eapply SModRed.interp_vis_pg
-      | vis (Choose _) _ =>
-          _hprogress prg; eapply SModRed.interp_vis_core
-      | vis (Take _) _ =>
-          _hprogress prg; eapply SModRed.interp_vis_core
-      | vis (IO _ _) _ =>
-          _hprogress prg; eapply SModRed.interp_vis_core
-      | assumeK _ _ =>
-          _hprogress prg; eapply SModRed.interp_assumeK
-      | guaranteeK _ _ =>
-          _hprogress prg; eapply SModRed.interp_guaranteeK
-      | unwrapUK _ _ =>
-          _hprogress prg; eapply SModRed.interp_unwrapUK
-      | unwrapNK _ _ =>
-          _hprogress prg; eapply SModRed.interp_unwrapNK
-      | _ =>
-          reflexivity
-      end
-  end.
-
-Tactic Notation "red_P" hyp(prg) :=
-  lazymatch goal with
-  | [ |- @PMod.interp _ _ ?itr = _ ] =>
-      lazymatch itr with
-      | Ret _ =>
-          _hprogress prg; eapply PModRed.interp_ret
-      | Tau _ =>
-          _hprogress prg; eapply PModRed.interp_tau
-      | vis (Spawn _ _) _ =>
-          _hprogress prg; eapply PModRed.interp_vis_sch
-      | vis (Yield _) _ =>
-          _hprogress prg; eapply PModRed.interp_vis_sch
-      | vis (Call _ _) _ =>
-          _hprogress prg; eapply PModRed.interp_vis_call
-      | vis (SPut _ _) _ =>
-          _hprogress prg; eapply PModRed.interp_vis_pg
-      | vis (SGet _) _ =>
-          _hprogress prg; eapply PModRed.interp_vis_pg
-      | vis (Choose _) _ =>
-          _hprogress prg; eapply PModRed.interp_vis_choose
-      | vis (Take _) _ =>
-          _hprogress prg; eapply PModRed.interp_vis_take
-      | vis (IO _ _) _ =>
-          _hprogress prg; eapply PModRed.interp_vis_io
-      | assumeK _ _ =>
-          _hprogress prg; eapply PModRed.interp_assumeK
-      | guaranteeK _ _ =>
-          _hprogress prg; eapply PModRed.interp_guaranteeK
-      | unwrapUK _ _ =>
-          _hprogress prg; eapply PModRed.interp_unwrapUK
-      | unwrapNK _ _ =>
-          _hprogress prg; eapply PModRed.interp_unwrapNK
-      | _ =>
-          reflexivity
-      end
-  end.
-
-Ltac _hnorm_itr prg :=
-  lazymatch goal with
-  | [ |- Ret _ = _ ] =>
-      reflexivity
-  | [ |- Tau _ = _ ] =>
-      reflexivity
-  | [ |- vis _ _ = _ ] =>
-      reflexivity
-  | [ |- @ITree.bind ?E ?T ?U ?itr ?ktr = _ ] =>
-      etransitivity;
-      [ let itr' := fresh "itr" in cong (fun itr' => @ITree.bind E T U itr' ktr); _hnorm_itr prg | red_bind prg (do 1 _hnorm_itr prg) ]
-  | [ |- @HMod.sandbox ?Σ ?R ?scopes ?itr = _ ] =>
-      etransitivity;
-      [ cong (@HMod.sandbox Σ R scopes); _hnorm_itr prg | red_SB prg ]
-  | [ |- @interp_smod ?Σ ?ginv ?stb ?R ?itr = _ ] =>
-      etransitivity;
-      [ cong (@interp_smod Σ ginv stb R); _hnorm_itr prg | red_S prg (do 1 _hnorm_itr prg) ]
-  | [ |- @PMod.interp ?Σ ?R ?itr = _ ] =>
-      etransitivity;
-      [ cong (@PMod.interp Σ R); _hnorm_itr prg | red_P prg ]
-  | [ |- trigger _ = _ ] =>
-      eapply trigger_vis
-  | [ |- assume _ = _ ] =>
-      eapply assume_assumeK
-  | [ |- guarantee _ = _ ] =>
-      eapply guarantee_guaranteeK
-  | [ |- unwrapU _ = _ ] =>
-      eapply unwrapU_unwrapUK
-  | [ |- unwrapN _ = _ ] =>
-      eapply unwrapN_unwrapNK
-  | [ |- HoareCall _ _ _ = _ ] =>
-      _hprogress prg; unfold HoareCall;
-      _hnorm_itr prg
-  | [ |- HoareSpawn _ _ _ _ = _ ] =>
-      _hprogress prg; unfold HoareSpawn;
-      _hnorm_itr prg
-  | [ |- HoareYield _ _ = _ ] =>
-      _hprogress prg; unfold HoareYield;
-      _hnorm_itr prg
-  | [ |- fbody_trivial _ = _ ] =>
-      _hprogress prg; unfold fbody_trivial;
-      _hnorm_itr prg
-  | [ |- cput _ _ = _ ] =>
-      _hprogress prg; unfold cput;
-      _hnorm_itr prg
-  | [ |- cgetU _ = _ ] =>
-      _hprogress prg; unfold cgetU;
-      _hnorm_itr prg
-  | [ |- cgetN _ = _ ] =>
-      _hprogress prg; unfold cgetN;
-      _hnorm_itr prg
-  | [ |- cfunU _ _ = _ ] =>
-      _hprogress prg; unfold cfunU;
-      _hnorm_itr prg
-  | [ |- cfunN _ _ = _ ] =>
-      _hprogress prg; unfold cfunN;
-      _hnorm_itr prg
-  | [ |- ccallU _ _ = _ ] =>
-      _hprogress prg; unfold ccallU;
-      _hnorm_itr prg
-  | [ |- ccallN _ _ = _ ] =>
-      _hprogress prg; unfold ccallN;
-      _hnorm_itr prg
-  | [ |- triggerUB = _ ] =>
-      _hprogress prg; unfold triggerUB;
-      _hnorm_itr prg
-  | [ |- triggerNB = _ ] =>
-      _hprogress prg; unfold triggerNB;
-      _hnorm_itr prg
-  | [ |- ?itr = _ ] =>
-      reflexivity
-  end.
-
-Ltac hnorm_itr :=
-  try match goal with
-  | [ |- @ITree.bind _ _ _ (trigger _) _ = _ ] => fail 2
-  end;
-  let prg := fresh "Progress" in
-  epose (prg := _ : _hprogress);
-  etransitivity;
-  [ _hnorm_itr prg
-  | _hprogress_check prg; s;
-    lazymatch goal with
-    | [ |- Ret _ = _ ] =>
-        reflexivity
-    | [ |- Tau _ = _ ] =>
-        reflexivity
-    | [ |- vis _ _ = _ ] =>
-        eapply vis_trigger
-    | [ |- assumeK _ _ = _ ] =>
-        eapply assumeK_assume
-    | [ |- guaranteeK _ _ = _ ] =>
-        eapply guaranteeK_guarantee
-    | [ |- unwrapUK _ _ = _ ] =>
-        eapply unwrapUK_unwrapU
-    | [ |- unwrapNK _ _ = _ ] =>
-        eapply unwrapNK_unwrapN
-    | [ |- HModSB.putSB _ _ _ _ = _ ] =>
-        eapply HModSB.putSB_SPut
-    | [ |- HModSB.getSB _ _ _ = _ ] =>
-        eapply HModSB.getSB_SGet
-    | [ |- _ = _ ] =>
-        reflexivity
-    end
-  ].
-
-Ltac replace_l :=
-  lazymatch goal with
-  | [ |- environments.envs_entails ?env (isim ?is_closed ?fl_src ?tl_tgt ?Ist ?r ?g ?RR ?ps ?pt ?nths (?st_src, ?itr_src) (?st_tgt, ?itr_tgt)) ] =>
-      refine (eq_ind_r (fun itr_src' => environments.envs_entails env (isim is_closed fl_src tl_tgt Ist r g RR ps pt nths (st_src, itr_src') (st_tgt, itr_tgt))) _ _); cycle 1
-  end.
-
-Ltac replace_r :=
-  lazymatch goal with
-  | [ |- environments.envs_entails ?env (isim ?is_closed ?fl_src ?tl_tgt ?Ist ?r ?g ?RR ?ps ?pt ?nths (?st_src, ?itr_src) (?st_tgt, ?itr_tgt)) ] =>
-      refine (eq_ind_r (fun itr_tgt' => environments.envs_entails env (isim is_closed fl_src tl_tgt Ist r g RR ps pt nths (st_src, itr_src) (st_tgt, itr_tgt'))) _ _); cycle 1
-  end.
-
-Ltac hnorm_l := replace_l; [s; hnorm_itr|].
-Ltac hnorm_r := replace_r; [s; hnorm_itr|].
-
-(***
-  Step-level tactics
- ***)
-
-Ltac iIntrosFresh H := iIntros H || iIntrosFresh (H ++ "'")%string.
-
-Ltac des_pairs :=
-  (hrepeat do 1
-    match goal with
-    | [H: context[let () := ?x in _] |- _] =>
-        match type of x with
-        | () => destruct x
-        | (_ * _)%type =>
-            let n0 := fresh "q" in let n1 := fresh "q" in
-            let EQ := fresh "EQq" in
-            destruct x as [n0 n1] eqn: EQ
-        end
-    | |- context[let () := ?x in _] =>
-        match type of x with
-        | () => destruct x
-        | (_ * _)%type =>
-            let n0 := fresh "q" in let n1 := fresh "q" in
-            let EQ := fresh "EQq" in
-            destruct x as [n0 n1] eqn: EQ
-        end
-    end);
-   subst.
-
-Ltac desugar itr :=
-  match itr with
-  | fbody_trivial _ => rewrite {1}/itr
-  | HoareCall _ _ _ => rewrite {1}/itr
-  | HoareSpawn _ _ _ => rewrite {1}/itr
-  | HoareYield _ _ => rewrite {1}/itr
-  | cput _ _ => rewrite{1}/itr
-  | cgetU _ => rewrite{1}/itr
-  | cgetN _ => rewrite{1}/itr
-  | triggerUB => rewrite{1}/itr
-  | triggerNB => rewrite{1}/itr
-  end.
-
-Ltac _unwrapSB itr :=
-  match itr with
-  | Ret _ =>
-      rewrite HModSB.transl_ret
-  | tau;; _ =>
-      rewrite HModSB.transl_tau
-  | trigger (Choose _) => 
-      rewrite HModSB.transl_core
-  | trigger (Take _) => 
-      rewrite HModSB.transl_core
-  | trigger (IO _ _) => 
-      rewrite HModSB.transl_core  
-  | trigger (Call _ _) =>
-      rewrite HModSB.transl_call
-  | trigger (SPut _ _) =>
-      idtac
-  | trigger (SGet _) =>
-      idtac
-  | trigger (Assume _) => 
-      rewrite HModSB.transl_ag
-  | trigger (Guarantee _) => 
-      rewrite HModSB.transl_ag
-  | unwrapU _ =>
-      rewrite HModSB.transl_unwrapU
-  | unwrapN _ =>
-      rewrite HModSB.transl_unwrapN
-  | assume _ =>
-      rewrite HModSB.transl_asm
-  | guarantee _ =>
-      rewrite HModSB.transl_guar
-  | trigger (Spawn _ _) =>
-      rewrite HModSB.transl_sch
-  | trigger (Yield _) =>
-      rewrite HModSB.transl_sch
-  | _ => fail
-  end.
-
-Ltac unwrapSB :=
-  try match goal with
-  | [|-context[HMod.sandbox _ ?itr]] => first [desugar itr|fail 2]
-  end;
-  match goal with
-  | [|-context[HMod.sandbox _ (?itr >>= _)]] =>
-      rewrite HModSB.transl_bind; unwrapSB
-  | [|-context[HMod.sandbox _ ?itr]] => first [_unwrapSB itr|fail 2]
-  end.
-
-Ltac _unwrapS itr :=
-  match itr with
-  | Ret _ =>
-      rewrite SModRed.interp_ret
-  | tau;; _ =>
-      rewrite SModRed.interp_tau
-  | trigger (Choose _) => 
-      rewrite SModRed.interp_core
-  | trigger (Take _) => 
-      rewrite SModRed.interp_core
-  | trigger (IO _ _) => 
-      rewrite SModRed.interp_core  
-  | trigger (Call _ _) =>
-      rewrite SModRed.interp_call {1}/handle_callE_hmodE
-  | trigger (Spawn _ _) =>
-      rewrite SModRed.interp_sch {1}/handle_schE_hmodE
-  | trigger (Yield _) =>
-      rewrite SModRed.interp_sch {1}/handle_schE_hmodE
-  | trigger (SPut _ _) =>
-      rewrite SModRed.interp_pg
-  | trigger (SGet _) =>
-      rewrite SModRed.interp_pg
-  | trigger (Assume _) => 
-      rewrite SModRed.interp_ag
-  | trigger (Guarantee _) => 
-      rewrite SModRed.interp_ag
-  | unwrapU _ =>
-      rewrite SModRed.interp_unwrapU
-  | unwrapN _ =>
-      rewrite SModRed.interp_unwrapN
-  | assume _ =>
-      rewrite SModRed.interp_asm
-  | guarantee _ =>
-      rewrite SModRed.interp_guar
-  | _ => fail
-  end.
-
-Ltac unwrapS :=
-  try match goal with
-    | [|-context[interp_smod _ _ ?itr]] => first [desugar itr|fail 2]
-  end;
-  match goal with
-  | [|-context[interp_smod _ _ (?itr >>= _)]] =>
-      rewrite SModRed.interp_bind; unwrapS
-  | [|-context[interp_smod _ _ ?itr]] => first [_unwrapS itr|fail 2]
-  end.
-
-Ltac _unwrapP itr :=
-  match itr with
-  | Ret _ =>
-      rewrite PModRed.interp_ret
-  | tau;; _ =>
-      rewrite PModRed.interp_tau
-  | trigger (Choose _) => 
-      rewrite PModRed.interp_choose
-  | trigger (Take _) => 
-      rewrite PModRed.interp_take
-  | trigger (IO _ _) => 
-      rewrite PModRed.interp_io
-  | trigger (Call _ _) =>
-      rewrite PModRed.interp_call
-  | trigger (Spawn _ _) =>
-      rewrite PModRed.interp_sch
-  | trigger (Yield _) =>
-      rewrite PModRed.interp_sch
-  | trigger (SPut _ _) =>
-      rewrite PModRed.interp_pg
-  | trigger (SGet _) =>
-      rewrite PModRed.interp_pg
-  | unwrapU _ =>
-      rewrite PModRed.interp_unwrapU
-  | unwrapN _ =>
-      rewrite PModRed.interp_unwrapN
-  | assume _ =>
-      rewrite PModRed.interp_asm
-  | guarantee _ =>
-      rewrite PModRed.interp_guar
-  | _ => fail
-  end.
-
-Ltac unwrapP :=
-  try match goal with
-  | [|-context[PMod.interp ?itr]] => first [desugar itr|fail 2]
-  end;
-  match goal with
-  | [|-context[PMod.interp (?itr >>= _)]] =>
-      rewrite PModRed.interp_bind; unwrapP
-  | [|-context[PMod.interp ?itr]] => first [_unwrapP itr|fail 2]
-  end.
-
-Ltac has_precond_in TM :=
-  match goal with [H := ?P |- _] => match H with TM => match P with context[precond] => idtac end end end.
-Ltac has_postcond_in TM :=
-  match goal with [H := ?P |- _] => match H with TM => match P with context[postcond] => idtac end end end.
-Ltac unfold_precond_postcond term := let TM := fresh "_term" in
-  set (TM := term) at 1;
-  (hrepeat do 1 (has_precond_in TM; unfold precond in TM; simpl in TM));
-  (hrepeat do 1 (has_postcond_in TM; unfold postcond in TM; simpl in TM));
-  subst TM.
-
-Ltac _step_l :=
-  match goal with
-  (******* isim ******)
-  (** src **)
-  | [ |- environments.envs_entails _ (isim _ _ _ _ _ _ _ _ _ _ (_, tau;; _) _) ] =>
-      iApply isim_tau_src
-  | [ |- environments.envs_entails _ (isim _ _ _ _ _ _ _ _ _ _ (_, Ret _ >>= _) _) ] =>
-      rewrite bind_ret_l
-  | [ |- environments.envs_entails _ (isim _ _ _ _ _ _ _ _ _ _ (_, (HMod.sandbox _ (trigger (SPut _ _))) >>= _) _) ] =>
-      iApply isim_sput_src_sandbox; [s;eauto|]
-  | [ |- environments.envs_entails _ (isim _ _ _ _ _ _ _ _ _ _ (_, (HMod.sandbox _ (trigger (SGet _))) >>= _) _) ] =>
-      iApply isim_sget_src_sandbox; [s;eauto|]
-  | [ |- environments.envs_entails _ (isim _ _ _ _ _ _ _ _ _ _ (_, trigger (Take _) >>= _) _) ] =>
-      let name := fresh "q" in
-      iApply isim_take_src; iIntros (name)
-  | [ |- environments.envs_entails _ (isim _ _ _ _ _ _ _ _ _ _  (_, trigger (Assume ?P) >>= _) _) ] =>
-      unfold_precond_postcond P; iApply isim_Assume_src; iIntrosFresh "ASM"
-  | [ |- environments.envs_entails _ (isim _ _ _ _ _ _ _ _ _ _ (_, unwrapU ?ox >>= _) _) ] =>
-      let name := fresh "q" in
-      iApply isim_unwrapU_src; iIntros (name) "%";
-      match goal with [ H: ?x = Some _ |- _ ] => let G := fresh "G" in rename H into G; try rewrite -> G in * end
-  | [ |- environments.envs_entails _ (isim _ _ _ _ _ _ _ _ _ (_, assume _ >>= _) _) ] =>
-      let name := fresh "asm" in iApply isim_asm_src; iIntros (name)
-  end.
-
-Ltac _step_r :=
-  match goal with
-  (******* isim ******)
-  (** tgt **)
-  | [ |- environments.envs_entails _ (isim _ _ _ _ _ _ _ _ _ _ _ (_, Ret _ >>= _)) ] =>
-      rewrite bind_ret_l
-  | [ |- environments.envs_entails _ (isim _ _ _ _ _ _ _ _ _ _ _ (_, tau;; _)) ] =>
-      iApply isim_tau_tgt
-  | [ |- environments.envs_entails _ (isim _ _ _ _ _ _ _ _ _ _ _ (_, (HMod.sandbox _ (trigger (SPut _ _))) >>= _)) ] =>
-      iApply isim_sput_tgt_sandbox; [s; eauto|]
-  | [ |- environments.envs_entails _ (isim _ _ _ _ _ _ _ _ _ _ _ (_, (HMod.sandbox _ (trigger (SGet _))) >>= _)) ] =>
-      iApply isim_sget_tgt_sandbox; [s; eauto|]
-  | [ |- environments.envs_entails _ (isim _ _ _ _ _ _ _ _ _ _ _ (_, trigger (Choose _) >>= _)) ] =>
-      let name := fresh "q" in
-      iApply isim_choose_tgt; iIntros (name)
-  | [ |- environments.envs_entails _ (isim _ _ _ _ _ _ _ _ _ _ _ (_, trigger (Guarantee ?P) >>= _)) ] =>
-      unfold_precond_postcond P; iApply isim_Guarantee_tgt; iIntrosFresh "GRT"
-  | [ |- environments.envs_entails _ (isim _ _ _ _ _ _ _ _ _ _ _ (_, unwrapN ?ox >>= _)) ] =>
-      let name := fresh "q" in
-      iApply isim_unwrapN_tgt; iIntros (name) "%";
-      match goal with [ H: ?x = Some _ |- _ ] => let G := fresh "G" in rename H into G; try rewrite -> G in * end
-  | [ |- environments.envs_entails _ (isim _ _ _ _ _ _ _ _ _ _ _ (_, guarantee _ >>= _)) ] =>
-      let name := fresh "grt" in iApply isim_guar_tgt; iIntros (name)
-  end.
-
-Ltac _step :=
-  match goal with
-  (******* isim ******)
-  (** both **)
-  | [ |- environments.envs_entails _ (isim _ _ _ _ _ _ _ _ _ _ (_, Ret _) (_, Ret _)) ] =>
-      iApply isim_ret
-  | [ |- environments.envs_entails _ (isim _ _ _ _ _ _ _ _ _ _ (_, trigger (IO _ _) >>= _) (_, trigger (IO _ _) >>= _)) ] =>
-      iApply isim_io; iIntros "%"
-  | [ |- environments.envs_entails _ (isim _ _ _ _ _ _ _ _ _ _ (_, trigger (Spawn _ _) >>= _) (_, trigger (Spawn _ _) >>= _)) ] =>
-      iApply isim_spawn
-  end.
-
-Ltac _force_l :=
-  match goal with
-  | [ |- environments.envs_entails _ (isim _ _ _ _ _ _ _ _ _ _ (_, trigger (Choose ?T) >>= _) _) ] =>
-      iApply isim_choose_src
-  | [ |- environments.envs_entails _ (isim _ _ _ _ _ _ _ _ _ _ (_, trigger (Guarantee ?P) >>= _) _) ] =>
-      unfold_precond_postcond P; iApply isim_Guarantee_src
-  | [ |- environments.envs_entails _ (isim _ _ _ _ _ _ _ _ _ _ (_, unwrapN _ >>= _) _) ] =>
-      iApply isim_unwrapN_src; iExists _
-  | [ |- environments.envs_entails _ (isim _ _ _ _ _ _ _ _ _ _ (_, guarantee _ >>= _) _) ] =>
-      iApply isim_guar_src
-  end
-.
-
-Ltac _force_r :=
-  match goal with
-  | [ |- environments.envs_entails _ (isim _ _ _ _ _ _ _ _ _ _ _ (_, trigger (Take _) >>= _)) ] =>
-      iApply isim_take_tgt
-  | [ |- environments.envs_entails _ (isim _ _ _ _ _ _ _ _ _ _ _ (_, trigger (Assume ?P) >>= _)) ] =>
-      unfold_precond_postcond P; iApply isim_Assume_tgt
-  | [ |- environments.envs_entails _ (isim _ _ _ _ _ _ _ _ _ _ _ (_, unwrapU _ >>= _)) ] =>
-      iApply isim_unwrapU_tgt; iExists _
-  | [ |- environments.envs_entails _ (isim _ _ _ _ _ _ _ _ _ _ _ (_, assume _ >>= _)) ] =>
-      iApply isim_asm_tgt
-  end
-.
-
-Ltac set_marker marker :=
-  assert (marker: True) by exact I.
-
-Ltac hide_ihyps_env env :=
-  match env with
-  | environments.Enil => idtac
-  | environments.Esnoc ?tl _ ?hyp =>
-      hide_ihyps_env tl;
-      let IHYP := fresh "IHYP" in
-      set (IHYP := hyp) at 1
-  end.
-
-Ltac hide_ihyps :=
-  match goal with
-  | [ |- environments.envs_entails {|environments.env_intuitionistic := ?ienv; environments.env_spatial := ?env |} _] =>
-      hide_ihyps_env ienv;
-      hide_ihyps_env env
-  end.
-
-Ltac show_itree :=
-  match goal with [H:_|-_] => unfold H; clear H end.
-
-Ltac hide_itree_l :=
-  match goal with [|- _ (_ (_, ?it) _)] => set (IT := it) at 1 end.
-
-Ltac hide_itree_r :=
-  match goal with [|- _ (_ _ (_, ?it))] => first [set (IT := it) at 2|set (IT := it) at 1] end.
-
-Ltac show_until marker :=
-  (hrepeat do 1 match goal with
-      [H: _ |- _] =>
-        try match H with marker => fail 3 end;
-        first [unfold H; clear H | revert H]
-    end);
-  clear marker; i.
-
-Ltac unfold_spc :=
-  try match goal with
-    [|-context[unwrapN (?spc ?name)]] =>
-      try match goal with
-        [H: context[spc_incl _ spc]|-_] =>
-          let RW := fresh "_RW" in let ND := fresh "_ND" in
-          edestruct H as [ND RW];
-          erewrite (RW name);
-          [|revert ND; unfold to_spc;
-            match goal with [|-context[alist_find _ ?x]] => rewrite /x end;
-            unseal CRIS; i;
-            alist_find_simpl;
-            refl];
-          simpl unwrapN; clear ND RW
-      end
-  end.
-
-Ltac _prep :=
-  first
-    [ unwrapSB
-    | unwrapS; unfold_spc; unwrapSB
-    | unwrapP; unwrapSB
-    | idtac].
-
-Ltac prep :=
-  try rewrite !bind_bind;
-  try match goal with
-  | [|-context[interp_smod _ _ (?f ?arg)]] =>
-    match type of arg with Any.t => rewrite {1}/f end
-  | [|-context[PMod.interp (?f ?arg)]] =>
-    match type of arg with Any.t => rewrite {1}/f end
-  end;
-  unfold ccallU, ccallN;
-  try match goal with
-      | [|-context[(_, HMod.sandbox _ _)]] => _prep
-      | [|-context[(_, HMod.sandbox _ _ >>= _)]] => _prep
-      end;
-  try rewrite !bind_bind;
-  try rewrite !bind_tau.
-
-Ltac prep_l :=
-  let marker := fresh "MARKER" in
-  set_marker marker;
-  hide_ihyps;
-  hide_itree_r;
-  prep;
-  show_until marker.
-
-Ltac prep_r :=
-  let marker := fresh "MARKER" in
-  set_marker marker;
-  hide_ihyps;
-  hide_itree_l;
-  prep;
-  show_until marker.
-
-Ltac step_l_core :=
-  _step_l; try alist_find_simpl; s; des_pairs; s.
-
-Ltac step_l :=
-  let marker := fresh "MARKER" in
-  set_marker marker;
-  hide_ihyps;
-  (hrepeat do 1 hnorm_l);
-  try step_l_core;
-  show_until marker.
-
-Ltac steps_l :=
-  let marker := fresh "MARKER" in
-  set_marker marker;
-  hide_ihyps;
-  (hrepeat do 1 tryany (do 1 hnorm_l) (do 1 step_l_core)); try hnorm_l;
-  show_until marker.
-
-Ltac step_r_core :=
-  _step_r; try alist_find_simpl; s; des_pairs; s.
-
-Ltac step_r :=
-  let marker := fresh "MARKER" in
-  set_marker marker;
-  hide_ihyps;
-  (hrepeat do 1 hnorm_r);
-  try step_r_core;
-  show_until marker.
-
-Ltac steps_r :=
-  let marker := fresh "MARKER" in
-  set_marker marker;
-  hide_ihyps;
-  (hrepeat do 1 tryany (do 1 hnorm_r) (do 1 step_r_core)); try hnorm_r;
-  show_until marker.
-
-Ltac step :=
-  let marker := fresh "MARKER" in
-  set_marker marker;
-  hide_ihyps;
-  (hrepeat do 1 hnorm_l);
-  (hrepeat do 1 hnorm_r);
-  _step;
-  s; des_pairs; s;
-  show_until marker.
-
-Ltac force_l_core :=
-  let marker := fresh "MARKER" in
-  set_marker marker;
-  hide_ihyps;
-  (hrepeat do 1 hnorm_l);
-  _force_l; s;
-  show_until marker.
-
-Tactic Notation "force_l" :=
-  force_l_core; try (iExists _).
-
-Tactic Notation "force_l" uconstr(p) :=
-  force_l_core; iExists p.
-
-Ltac forces_l :=
-  hrepeat do 1 force_l.
-
-Ltac force_r_core :=
-  let marker := fresh "MARKER" in
-  set_marker marker;  
-  hide_ihyps;
-  (hrepeat do 1 hnorm_r);
-  _force_r; s;
-  show_until marker.
-
-Tactic Notation "force_r" :=
-  force_r_core; try (iExists _).
-
-Tactic Notation "force_r" uconstr(p) :=
-  force_r_core; iExists p.
-
-Ltac forces_r := hrepeat do 1 force_r.
-
-Ltac unfold_cris_defs :=
-  (hrepeat do 1 match goal with
-  | [|- context[{| fsb_body := cfunU ?x |}]] => rewrite {1}/x
-  | [|- context[{| fsb_body := cfunN ?x |}]] => rewrite {1}/x
-  | [|- context[{| fsb_body := ?x |}]] => rewrite {1}/x
-  | [|- context[PMod.interp (?x _)]] => unfold x
-  | [|- context[cfunU ?x]] => rewrite {1}/x
-  | [|- context[cfunN ?x]] => rewrite {1}/x
-  end);
-  unfold interp_sb_hp, HoareFun, cfunU, cfunN, HMod.sandbox_body; s.  
-
-Ltac prove_inline_cond :=
-  match goal with [|- alist_find _ ?FL = _] =>
-    rewrite /FL;
-    simpl HMod.fnsems; (hrepeat do 1 unfold_hmod);
-    simpl List.map; alist_find_simpl; eauto
-  end.
-
-Ltac inline_l :=
-  let marker := fresh "MARKER" in
-  set_marker marker;  
-  hide_ihyps;
-  (hrepeat do 1 hnorm_l);
-  iApply isim_inline_src; [prove_inline_cond|];
-  unfold_cris_defs;
-  show_until marker.
-  
-Ltac inline_r :=
-  let marker := fresh "MARKER" in
-  set_marker marker;  
-  hide_ihyps;
-  (hrepeat do 1 hnorm_r);
-  iApply isim_inline_tgt; [prove_inline_cond|];
-  unfold_cris_defs;
-  show_until marker.
-
-Ltac call hyps :=
-  let marker := fresh "MARKER" in
-  set_marker marker;
-  hide_ihyps;
-  (hrepeat do 1 hnorm_l);
-  (hrepeat do 1 hnorm_r);
-  iApply isim_call;
-  show_until marker;
-  iSplitL hyps; [ |iIntros "% % % % % %"; iIntrosFresh "IST"];
-  move_aux.
-
-Ltac yield hyps :=
-  let marker := fresh "MARKER" in
-  set_marker marker;  
-  hide_ihyps;
-  (hrepeat do 1 hnorm_l);
-  (hrepeat do 1 hnorm_r);
-  iApply isim_yield;
-  show_until marker;
-  iSplitL hyps; [ |iIntros "% % % % %"; iIntrosFresh "IST"];
-  move_aux.
-
-Ltac hide_flist :=
-  let FLS := fresh "FLS" in let FLT := fresh "FLT" in
-  match goal with [|- context[(isim_fsem ?fls ?flt _ _)]] =>
-    set (FLS := fls); set (FLT := flt)
-  end.
-
-Ltac pre_simF :=
-  unfold HSim.sim_fun; i;
-  match goal with [H: _|-_] => revert H end;
-  hide_flist.
-
-Ltac post_simF :=
-  eexists; split; [eauto|];
-  unfold_cris_defs;
-  ii; subst; iIntros "IST";
-  move_aux.
-
-Ltac init_simF :=
-  pre_simF;
-  alist_find_simpl;
-  let H := fresh "H" in intro H; inv H;
-  alist_find_simpl;
-  post_simF.
-
-Ltac prove_sub_perm :=  
-  i; try rewrite /HMod.scopes; s; (hrepeat do 1 unfold_hmod); s;
-  match goal with
-    [|-sub_perm ?x ?y] =>
-      match x with
-      | _ :: _ => idtac
-      | _ => try rewrite /x
-      end;
-      match y with
-      | _ :: _ => idtac
-      | _ => try rewrite /y
-      end
-  end;
-  (hrepeat do 1 s;
-   match goal with [|-sub_perm (?k::_) ?tgt] =>
-     let key := fresh "key" in
-     set (key := k);
-     match tgt with
-     |  context[?k'::_] =>
-          change k' with key;
-          eapply eq_ind; [|symmetry; Lauto_prepare; Lauto_find key; refl];
-          eapply (sub_perm_cancel [key] [])
-     end;
-     unfold key; clear key
-  end);
-  apply sub_perm_nil.
+Require Export ITacticsCommon.
 
 (**** TODO ****)
 (* A tactic to handle meta variables *)
 
 (************ User Notations **************)
 
+(*** TODO: 
+          What else should be displayed? 
+          Simplify (hide) k-trees
+
+***)
+
 From iris.proofmode Require Import coq_tactics environments.
 
 Global Arguments Envs _ _%_proof_scope _%_proof_scope _.
 Global Arguments Enil {_}.
 Global Arguments Esnoc {_} _%_proof_scope _%_string _%_I.
-
-Local Notation world_id := positive.
-Local Notation level := nat.
-
-(*** TODO: 
-          What else should be displayed? 
-n          Simplify (hide) k-trees
-
-***)
 
 (*** isim ***)
 Notation "E1 '------------------------------------------------------------------□' E2 '------------------------------------------------------------------∗' st_src st_tgt '-------------------------------isim-------------------------------' itr_src itr_tgt"
@@ -1078,3 +59,212 @@ Notation "E1 '------------------------------------------------------------------
   (environments.envs_entails (Envs E1 E2 _) (bi_wand P (isim _ _ _ _ _ _ _ _ _ _ (st_src, _) (st_tgt, _))))
     (at level 50, only printing,
      format "E1 '------------------------------------------------------------------□' '//' E2 '------------------------------------------------------------------∗' '//' st_src '//' st_tgt '//' '-------------------------------isim-------------------------------' '//' P  '-∗'  'ISIM' ").
+
+Ltac replace_l :=
+  lazymatch goal with
+  | [ |- environments.envs_entails ?env (isim ?is_closed ?fl_src ?tl_tgt ?Ist ?r ?g ?RR ?ps ?pt ?nths (?st_src, ?itr_src) (?st_tgt, ?itr_tgt)) ] =>
+      refine (eq_ind_r (fun itr_src' => environments.envs_entails env (isim is_closed fl_src tl_tgt Ist r g RR ps pt nths (st_src, itr_src') (st_tgt, itr_tgt))) _ _); cycle 1
+  end.
+
+Ltac replace_r :=
+  lazymatch goal with
+  | [ |- environments.envs_entails ?env (isim ?is_closed ?fl_src ?tl_tgt ?Ist ?r ?g ?RR ?ps ?pt ?nths (?st_src, ?itr_src) (?st_tgt, ?itr_tgt)) ] =>
+      refine (eq_ind_r (fun itr_tgt' => environments.envs_entails env (isim is_closed fl_src tl_tgt Ist r g RR ps pt nths (st_src, itr_src) (st_tgt, itr_tgt'))) _ _); cycle 1
+  end.
+
+Ltac hnorm_l := replace_l; [s; hnorm_itr|].
+Ltac hnorm_r := replace_r; [s; hnorm_itr|].
+
+Tactic Notation "hnorm_l" "with" tactic(tac) :=
+  let marker := fresh "MARKER" in
+  set_marker marker;
+  hide_ihyps;
+  (hrepeat do 1 hnorm_l);  
+  tac;
+  show_until marker.
+
+Tactic Notation "hnorm_r" "with" tactic(tac) :=
+  let marker := fresh "MARKER" in
+  set_marker marker;
+  hide_ihyps;
+  (hrepeat do 1 hnorm_r);  
+  tac;
+  show_until marker.
+
+Tactic Notation "hnorm" "with" tactic(tac) :=
+  let marker := fresh "MARKER" in
+  set_marker marker;
+  hide_ihyps;
+  (hrepeat do 1 hnorm_l);
+  (hrepeat do 1 hnorm_r);
+  tac;
+  show_until marker.
+
+(***
+  Step-level tactics
+ ***)
+
+Ltac _step_l :=
+  match goal with
+  (******* isim ******)
+  (** src **)
+  | [ |- environments.envs_entails _ (isim _ _ _ _ _ _ _ _ _ _ (_, tau;; _) _) ] =>
+      iApply isim_tau_src
+  | [ |- environments.envs_entails _ (isim _ _ _ _ _ _ _ _ _ _ (_, Ret _ >>= _) _) ] =>
+      rewrite bind_ret_l
+  | [ |- environments.envs_entails _ (isim _ _ _ _ _ _ _ _ _ _ (_, (HMod.sandbox _ (trigger (SPut _ _))) >>= _) _) ] =>
+      iApply isim_sput_src_sandbox; [s;eauto|]
+  | [ |- environments.envs_entails _ (isim _ _ _ _ _ _ _ _ _ _ (_, (HMod.sandbox _ (trigger (SGet _))) >>= _) _) ] =>
+      iApply isim_sget_src_sandbox; [s;eauto|]
+  | [ |- environments.envs_entails _ (isim _ _ _ _ _ _ _ _ _ _ (_, trigger (Take _) >>= _) _) ] =>
+      let name := fresh "q" in
+      iApply isim_take_src; iIntros (name)
+  | [ |- environments.envs_entails _ (isim _ _ _ _ _ _ _ _ _ _  (_, trigger (Assume ?P) >>= _) _) ] =>
+      unfold_precond_postcond P; iApply isim_Assume_src; iIntrosFresh "ASM"
+  | [ |- environments.envs_entails _ (isim _ _ _ _ _ _ _ _ _ _ (_, unwrapU ?ox >>= _) _) ] =>
+      let name := fresh "q" in
+      iApply isim_unwrapU_src; iIntros (name) "%";
+      match goal with [ H: ?x = Some _ |- _ ] => let G := fresh "G" in rename H into G; try rewrite -> G in * end
+  | [ |- environments.envs_entails _ (isim _ _ _ _ _ _ _ _ _ (_, assume _ >>= _) _) ] =>
+      let name := fresh "asm" in iApply isim_asm_src; iIntros (name)
+  end.
+
+Ltac step_l_core :=
+  _step_l; try alist_find_simpl; s; des_pairs; s.
+
+Ltac step_l :=
+  hnorm_l with do 1 try step_l_core.
+
+Ltac steps_l :=
+  let marker := fresh "MARKER" in
+  set_marker marker;
+  hide_ihyps;
+  (hrepeat do 1 tryany (do 1 hnorm_l) (do 1 step_l_core)); try hnorm_l;
+  show_until marker.
+
+Ltac _step_r :=
+  match goal with
+  (******* isim ******)
+  (** tgt **)
+  | [ |- environments.envs_entails _ (isim _ _ _ _ _ _ _ _ _ _ _ (_, Ret _ >>= _)) ] =>
+      rewrite bind_ret_l
+  | [ |- environments.envs_entails _ (isim _ _ _ _ _ _ _ _ _ _ _ (_, tau;; _)) ] =>
+      iApply isim_tau_tgt
+  | [ |- environments.envs_entails _ (isim _ _ _ _ _ _ _ _ _ _ _ (_, (HMod.sandbox _ (trigger (SPut _ _))) >>= _)) ] =>
+      iApply isim_sput_tgt_sandbox; [s; eauto|]
+  | [ |- environments.envs_entails _ (isim _ _ _ _ _ _ _ _ _ _ _ (_, (HMod.sandbox _ (trigger (SGet _))) >>= _)) ] =>
+      iApply isim_sget_tgt_sandbox; [s; eauto|]
+  | [ |- environments.envs_entails _ (isim _ _ _ _ _ _ _ _ _ _ _ (_, trigger (Choose _) >>= _)) ] =>
+      let name := fresh "q" in
+      iApply isim_choose_tgt; iIntros (name)
+  | [ |- environments.envs_entails _ (isim _ _ _ _ _ _ _ _ _ _ _ (_, trigger (Guarantee ?P) >>= _)) ] =>
+      unfold_precond_postcond P; iApply isim_Guarantee_tgt; iIntrosFresh "GRT"
+  | [ |- environments.envs_entails _ (isim _ _ _ _ _ _ _ _ _ _ _ (_, unwrapN ?ox >>= _)) ] =>
+      let name := fresh "q" in
+      iApply isim_unwrapN_tgt; iIntros (name) "%";
+      match goal with [ H: ?x = Some _ |- _ ] => let G := fresh "G" in rename H into G; try rewrite -> G in * end
+  | [ |- environments.envs_entails _ (isim _ _ _ _ _ _ _ _ _ _ _ (_, guarantee _ >>= _)) ] =>
+      let name := fresh "grt" in iApply isim_guar_tgt; iIntros (name)
+  end.
+
+Ltac step_r_core :=
+  _step_r; try alist_find_simpl; s; des_pairs; s.
+
+Ltac step_r :=
+  hnorm_r with do 1 try step_r_core.
+
+Ltac steps_r :=
+  let marker := fresh "MARKER" in
+  set_marker marker;
+  hide_ihyps;
+  (hrepeat do 1 tryany (do 1 hnorm_r) (do 1 step_r_core)); try hnorm_r;
+  show_until marker.
+
+Ltac _step :=
+  match goal with
+  (******* isim ******)
+  (** both **)
+  | [ |- environments.envs_entails _ (isim _ _ _ _ _ _ _ _ _ _ (_, Ret _) (_, Ret _)) ] =>
+      iApply isim_ret
+  | [ |- environments.envs_entails _ (isim _ _ _ _ _ _ _ _ _ _ (_, trigger (IO _ _) >>= _) (_, trigger (IO _ _) >>= _)) ] =>
+      iApply isim_io; iIntros "%"
+  | [ |- environments.envs_entails _ (isim _ _ _ _ _ _ _ _ _ _ (_, trigger (Spawn _ _) >>= _) (_, trigger (Spawn _ _) >>= _)) ] =>
+      iApply isim_spawn
+  end.
+
+Ltac step :=
+  hnorm with do 1 _step; s; des_pairs; s.
+
+Ltac _force_l :=
+  match goal with
+  | [ |- environments.envs_entails _ (isim _ _ _ _ _ _ _ _ _ _ (_, trigger (Choose ?T) >>= _) _) ] =>
+      iApply isim_choose_src
+  | [ |- environments.envs_entails _ (isim _ _ _ _ _ _ _ _ _ _ (_, trigger (Guarantee ?P) >>= _) _) ] =>
+      unfold_precond_postcond P; iApply isim_Guarantee_src
+  | [ |- environments.envs_entails _ (isim _ _ _ _ _ _ _ _ _ _ (_, unwrapN _ >>= _) _) ] =>
+      iApply isim_unwrapN_src; iExists _
+  | [ |- environments.envs_entails _ (isim _ _ _ _ _ _ _ _ _ _ (_, guarantee _ >>= _) _) ] =>
+      iApply isim_guar_src
+  end
+.
+
+Ltac force_l_core :=
+  hnorm_l with do 1 _force_l; s.
+
+Tactic Notation "force_l" :=
+  force_l_core; try (iExists _).
+
+Tactic Notation "force_l" uconstr(p) :=
+  force_l_core; iExists p.
+
+Ltac forces_l :=
+  hrepeat do 1 force_l.
+
+Ltac _force_r :=
+  match goal with
+  | [ |- environments.envs_entails _ (isim _ _ _ _ _ _ _ _ _ _ _ (_, trigger (Take _) >>= _)) ] =>
+      iApply isim_take_tgt
+  | [ |- environments.envs_entails _ (isim _ _ _ _ _ _ _ _ _ _ _ (_, trigger (Assume ?P) >>= _)) ] =>
+      unfold_precond_postcond P; iApply isim_Assume_tgt
+  | [ |- environments.envs_entails _ (isim _ _ _ _ _ _ _ _ _ _ _ (_, unwrapU _ >>= _)) ] =>
+      iApply isim_unwrapU_tgt; iExists _
+  | [ |- environments.envs_entails _ (isim _ _ _ _ _ _ _ _ _ _ _ (_, assume _ >>= _)) ] =>
+      iApply isim_asm_tgt
+  end
+.
+
+Ltac force_r_core :=
+  hnorm_r with do 1 _force_r; s.
+
+Tactic Notation "force_r" :=
+  force_r_core; try (iExists _).
+
+Tactic Notation "force_r" uconstr(p) :=
+  force_r_core; iExists p.
+
+Ltac forces_r := hrepeat do 1 force_r.
+
+Ltac inline_l :=
+  hnorm_l with
+    do 1 iApply isim_inline_src; [prove_inline_cond|]; unfold_cris_defs.
+
+Ltac inline_r :=
+  hnorm_r with
+    do 1 iApply isim_inline_tgt; [prove_inline_cond|]; unfold_cris_defs.
+
+Ltac call hyps :=
+  (hnorm with do 1 iApply isim_call);
+  iSplitL hyps; [ |iIntros "% % % % % %"; iIntrosFresh "IST"];
+  move_aux.
+
+Ltac yield hyps :=
+  (hnorm with do 1 iApply isim_yield);
+  iSplitL hyps; [ |iIntros "% % % % %"; iIntrosFresh "IST"];
+  move_aux.
+
+Ltac by_coind CIH :=
+  iApply isim_progress; iApply isim_base;
+  iSpecialize (CIH $! _);
+  (hrepeat do 1 first[instantiate (1:= (_,_))|instantiate (1:= existT _ _)]); s;
+  iApply CIH.
+
